ground type inferwidth proof2

src/InferWidthsnew.v
@@ -27,7 +27,7 @@ Fixpoint ft_find_sub (checkt : ftype) (num : N) : option fgtyp :=
 with ft_find_ff (ff : ffield) (num : N) : option fgtyp :=
   match ff with
   | Fflips v0 _ ft ff' => if num >= (N.of_nat (tmap_type_size ft)) (* 不在该field中, 找下一个field *)
-                              then ft_find_ff ff' (N.sub num (N.of_nat (num_ref ft)))
+                              then ft_find_ff ff' (N.sub num (N.of_nat (tmap_type_size ft)))
                            else (* 在field v0中 *)
                               ft_find_sub ft num
   | _ => None
@@ -42,11 +42,11 @@ Fixpoint ft_check_flip (checkt : ftype) (num : N) (fl : bool) : option bool :=
 with ft_check_flip_f (ff : ffield) (num : N) (fl : bool) : option bool :=
   match ff with
   | Fflips v0 Flipped ft ff' => if num >= (N.of_nat (tmap_type_size ft)) (* 不在该field中, 找下一个field *)
-                                  then ft_check_flip_f ff' (N.sub num (N.of_nat (num_ref ft))) fl
+                                  then ft_check_flip_f ff' (N.sub num (N.of_nat (tmap_type_size ft))) fl
                               else (* 在field v0中 *)
                                   ft_check_flip ft num (~~fl)
   | Fflips v0 Nflip ft ff' => if num >= (N.of_nat (tmap_type_size ft)) (* 不在该field中, 找下一个field *)
-                                  then ft_check_flip_f ff' (N.sub num (N.of_nat (num_ref ft))) fl
+                                  then ft_check_flip_f ff' (N.sub num (N.of_nat (tmap_type_size ft))) fl
                               else (* 在field v0中 *)
                                   ft_check_flip ft num fl
   | _ => None
@@ -67,7 +67,7 @@ Fixpoint ft_set_sub (checkt : ftype) (newt : fgtyp) (num : N) : option ftype :=
   end
 with ft_set_sub_f (ff : ffield) (newt : fgtyp) (num : N) : option ffield :=
   match ff with
-  | Fflips v0 fl ft ff' => if N.to_nat num >= (tmap_type_size ft) (* 不在该field中, 找下一个field *)
+  | Fflips v0 fl ft ff' => if num >= N.of_nat (tmap_type_size ft) (* 不在该field中, 找下一个field *)
                             then match ft_set_sub_f ff' newt (N.sub num (N.of_nat (tmap_type_size ft))) with
                                 | Some newf => Some (Fflips v0 fl ft newf)
                                 | None => None
@@ -109,13 +109,28 @@ Definition ports_tmap (ps : seq HiFP.hfport) : CEP.t ftype :=
 seq.foldl port_tmap (CEP.empty ftype) ps.
 
 (* type of mux expression *)
+Definition mux_gtyp (t1 : fgtyp) (t2 : fgtyp) : option fgtyp :=
+      match t1, t2 with
+      | Fuint w1, Fuint w2 => Some (Fuint (maxn w1 w2))
+      | Fuint w1, Fuint_implicit w2 => Some (Fuint (maxn w1 w2))
+      | Fuint_implicit w1, Fuint w2 => Some (Fuint (maxn w1 w2))
+      | Fuint_implicit w1, Fuint_implicit w2 => Some (Fuint (maxn w1 w2))
+      | Fsint w1, Fsint w2 => Some (Fsint (maxn w1 w2))
+      | Fsint w1, Fsint_implicit w2 => Some (Fsint (maxn w1 w2))
+      | Fsint_implicit w1, Fsint w2 => Some (Fsint (maxn w1 w2))
+      | Fsint_implicit w1, Fsint_implicit w2 => Some (Fsint (maxn w1 w2))
+      | Fclock, Fclock => Some (Fclock)
+      | Freset, Freset => Some (Freset)
+      | Fasyncreset, Fasyncreset => Some (Fasyncreset)
+      | _,_ => None
+      end.
+
 Fixpoint mux_types (t1 : ftype) (t2 : ftype) : option ftype :=
       match t1, t2 with
-      | Gtyp (Fuint w1), Gtyp (Fuint w2) => Some (Gtyp (Fuint (maxn w1 w2)))
-      | Gtyp (Fsint w1), Gtyp (Fsint w2) => Some (Gtyp (Fsint (maxn w1 w2)))
-      | Gtyp Fclock, Gtyp Fclock => Some (Gtyp Fclock)
-      | Gtyp Freset, Gtyp Freset => Some (Gtyp Freset)
-      | Gtyp Fasyncreset, Gtyp Fasyncreset => Some (Gtyp Fasyncreset)
+      | Gtyp gt1, Gtyp gt2 => match mux_gtyp gt1 gt2 with
+                              | Some gt => Some (Gtyp gt)
+                              | _ => None
+                              end
       | Atyp t1' n1, Atyp t2' n2 => match n1 == n2, mux_types t1' t2' with
                                     | true, Some t => Some (Atyp t n1)
                                     | _, _ => None
@@ -384,7 +399,7 @@ match e with
                             | _, _ => None
                             end
 | Emux c e1 e2 => match type_of_hfexpr c ce, type_of_hfexpr e1 ce, type_of_hfexpr e2 ce with
-                  | Some (Gtyp (Fuint 1)), Some t1, Some t2
+                  | Some (Gtyp (Fuint 1)), Some t1, Some t2 => mux_types t1 t2
                   | Some (Gtyp (Fuint_implicit 1)), Some t1, Some t2 =>
                       mux_types t1 t2
                   | _, _, _ => None
@@ -393,126 +408,6 @@ match e with
                    | Some (Gtyp (Fuint 1)) | Some (Gtyp (Fuint_implicit 1)) => type_of_hfexpr e1 ce
                    | _ => None
                    end
-end.
-
-Fixpoint tmap_add_bidir_connect (m_nt_ns : var2exprsmap * N * N) (v_tgt : VarOrder.t) (ref_tgt : HiFP.href) (t_tgt : ftype) (v_src : VarOrder.t) (ref_src : HiFP.href) (t_src : ftype) : option (var2exprsmap * N * N) :=
-(* check whether types are compatible and add connections for all ground-type entries of ref_tgt <= ref_src,
-   while taking into account flipped fields.
-   This works for InferWidths, so for arrays it only adds one connection, not one connection per entry.
-   m_n is a pair: a var2exprsmap to which connections are added
-                  a natural number that indicates which index of ref_tgt and ref_src is to be connected
-   v_tgt and v_src are variable names.
-   ref_tgt and ref_src are the respective hrefs that correspond to (v_tgt, m_nt_ns.1.2) and (v_src, m_nt_ns.2).
-   The return value is a triple where the first element is the updated var2exprsmap and
-   the second and third is increased by as many connections as there have been added. *)
-match t_tgt, t_src with
-| Gtyp (Fuint _), Gtyp (Fuint _) | Gtyp (Fuint _), Gtyp (Fuint_implicit _)
-| Gtyp (Fsint _), Gtyp (Fsint _) | Gtyp (Fsint _), Gtyp (Fsint_implicit _)
-| Gtyp Fclock, Gtyp Fclock
-| Gtyp Freset, Gtyp Freset
-| Gtyp Fasyncreset, Gtyp Fasyncreset =>
-    (* the target has explicit width, do not register the connection *)
-    Some (m_nt_ns.1.1, (m_nt_ns.1.2 + 1)%num, (m_nt_ns.2 + 1)%num)
-| Gtyp (Fuint_implicit _), Gtyp (Fuint _) | Gtyp (Fuint_implicit _), Gtyp (Fuint_implicit _)
-| Gtyp (Fsint_implicit _), Gtyp (Fsint _) | Gtyp (Fsint_implicit _), Gtyp (Fsint_implicit _) =>
-    Some (match module_graph_vertex_set_p.find (v_tgt, m_nt_ns.1.2) m_nt_ns.1.1 with
-          | Some expr_list => module_graph_vertex_set_p.add (v_tgt, m_nt_ns.1.2)    (Eref ref_src :: expr_list) m_nt_ns.1.1
-          | None =>           module_graph_vertex_set_p.add (v_tgt, m_nt_ns.1.2) [:: Eref ref_src]              m_nt_ns.1.1
-          end, (m_nt_ns.1.2 + 1)%num, (m_nt_ns.2 + 1)%num)
-| Atyp t_tgt' n_tgt, Atyp t_src' n_src =>
-    if n_tgt != n_src then None
-    else tmap_add_bidir_connect m_nt_ns v_tgt (Esubindex ref_tgt 0) t_tgt' v_src (Esubindex ref_src 0) t_src'
-| Btyp ff_tgt, Btyp ff_src => tmap_add_bidir_connect_fields m_nt_ns v_tgt ref_tgt ff_tgt v_src ref_src ff_src
-| _, _ => None
-end
-with tmap_add_bidir_connect_fields (m_nt_ns : var2exprsmap * N * N) (v_tgt : VarOrder.t) (ref_tgt : HiFP.href) (ff_tgt : ffield) (v_src : VarOrder.t) (ref_src : HiFP.href) (ff_src : ffield) : option (var2exprsmap * N * N) :=
-(* check whether types are compatible and add connections for all ground-type entries of ref_tgt <= ref_src,
-   where these are bundle types with types (Btyp ff_tgt) and (Btyp ff_src), respectively. *)
-match ff_tgt, ff_src with
-| Fnil, Fnil => Some m_nt_ns
-| Fflips v_tgt Nflip t_tgt ff_tgt', Fflips v_src Nflip t_src ff_src' =>
-    if v_tgt != v_src then None
-    else if tmap_add_bidir_connect m_nt_ns v_tgt (Esubfield ref_tgt v_tgt) t_tgt v_src (Esubfield ref_src v_src) t_src is Some m_nt_ns'
-         then tmap_add_bidir_connect_fields m_nt_ns' v_tgt ref_tgt ff_tgt' v_src ref_src ff_src'
-         else None
-| Fflips v_tgt Flipped t_tgt ff_tgt', Fflips v_src Flipped t_src ff_src' =>
-    if v_tgt != v_src then None
-    else if tmap_add_bidir_connect_flipped m_nt_ns v_tgt (Esubfield ref_tgt v_tgt) t_tgt v_src (Esubfield ref_src v_src) t_src is Some m_nt_ns'
-         then tmap_add_bidir_connect_fields m_nt_ns' v_tgt ref_tgt ff_tgt' v_src ref_src ff_src'
-         else None
-| _, _ => None
-end
-with tmap_add_bidir_connect_flipped (m_nt_ns : var2exprsmap * N * N) (v_tgt : VarOrder.t) (ref_tgt : HiFP.href) (t_tgt : ftype) (v_src : VarOrder.t) (ref_src : HiFP.href) (t_src : ftype) : option (var2exprsmap * N * N) :=
-(* check whether types are compatible and add connections for all ground-type entries of ref_src <= ref_tgt,
-   i.e. the other direction than tmap_add_bidir_connect. *)
-match t_tgt, t_src with
-| Gtyp (Fuint _), Gtyp (Fuint _) | Gtyp (Fuint_implicit _), Gtyp (Fuint _)
-| Gtyp (Fsint _), Gtyp (Fsint _) | Gtyp (Fsint_implicit _), Gtyp (Fsint _)
-| Gtyp Fclock, Gtyp Fclock
-| Gtyp Freset, Gtyp Freset
-| Gtyp Fasyncreset, Gtyp Fasyncreset =>
-    (* the target has explicit width, do not register the connection *)
-    Some (m_nt_ns.1.1, (m_nt_ns.1.2 + 1)%num, (m_nt_ns.2 + 1)%num)
-| Gtyp (Fuint _), Gtyp (Fuint_implicit _) | Gtyp (Fuint_implicit _), Gtyp (Fuint_implicit _)
-| Gtyp (Fsint _), Gtyp (Fsint_implicit _) | Gtyp (Fsint_implicit _), Gtyp (Fsint_implicit _) =>
-    Some (match module_graph_vertex_set_p.find (v_src, m_nt_ns.2) m_nt_ns.1.1 with
-          | Some expr_list => module_graph_vertex_set_p.add (v_src, m_nt_ns.2)    (Eref ref_tgt :: expr_list) m_nt_ns.1.1
-          | None =>           module_graph_vertex_set_p.add (v_src, m_nt_ns.2) [:: Eref ref_tgt]              m_nt_ns.1.1
-          end, (m_nt_ns.1.2 + 1)%num, (m_nt_ns.2 + 1)%num)
-| Atyp t_tgt' n_tgt, Atyp t_src' n_src =>
-    if n_tgt != n_src then None
-    else tmap_add_bidir_connect_flipped m_nt_ns v_tgt (Esubindex ref_tgt 0) t_tgt' v_src (Esubindex ref_src 0) t_src'
-| Btyp ff_tgt, Btyp ff_src => tmap_add_bidir_connect_flipped_fields m_nt_ns v_tgt ref_tgt ff_tgt v_src ref_src ff_src
-| _, _ => None
-end
-with tmap_add_bidir_connect_flipped_fields (m_nt_ns : var2exprsmap * N * N) (v_tgt : VarOrder.t) (ref_tgt : HiFP.href) (ff_tgt : ffield) (v_src : VarOrder.t) (ref_src : HiFP.href) (ff_src : ffield) : option (var2exprsmap * N * N) :=
-(* check whether types are compatible and add connections for all ground-type entries of ref_src <= ref_tgt,
-   where these are bundle types with types (Btyp ff_src) and (Btyp ff_tgt), respectively,
-   i.e. the other direction than tmap_add_bidir_connect_fields. *)
-match ff_tgt, ff_src with
-| Fnil, Fnil => Some m_nt_ns
-| Fflips v_tgt Nflip t_tgt ff_tgt', Fflips v_src Nflip t_src ff_src' =>
-    if v_tgt != v_src then None
-    else if tmap_add_bidir_connect_flipped m_nt_ns v_tgt (Esubfield ref_tgt v_tgt) t_tgt v_src (Esubfield ref_src v_src) t_src is Some m_nt_ns'
-         then tmap_add_bidir_connect_flipped_fields m_nt_ns' v_tgt ref_tgt ff_tgt' v_src ref_src ff_src'
-         else None
-| Fflips v_tgt Flipped t_tgt ff_tgt', Fflips v_src Flipped t_src ff_src' =>
-    if v_tgt != v_src then None
-    else if tmap_add_bidir_connect m_nt_ns v_tgt (Esubfield ref_tgt v_tgt) t_tgt v_src (Esubfield ref_src v_src) t_src is Some m_nt_ns'
-         then tmap_add_bidir_connect_flipped_fields m_nt_ns' v_tgt ref_tgt ff_tgt' v_src ref_src ff_src'
-         else None
-| _, _ => None
-end.
-
-Fixpoint tmap_add_passive_connect (m_nt : var2exprsmap * N) (v_tgt : VarOrder.t) (ref_src : HiFP.href) (t : ftype) : option (var2exprsmap * N) :=
-(* passive version of tmap_add_bidir_connect.
-   This works for InferWidths, so for arrays it only adds one connection, not one connection per entry.
-   m_nt is a pair: a var2exprsmap to which connections are added
-                  a natural number that indicates which index of ref_tgt and ref_src is to be connected
-   v_tgt is the variable name.
-   ref_src is the href that v_tgt is connected to.
-   The return value is a pair where the first element is the updated var2exprsmap and
-   the second element is increased by as many connections as there have been added. *)
-match t with
-| Gtyp (Fuint_implicit _)
-| Gtyp (Fsint_implicit _) =>
-    match module_graph_vertex_set_p.find (v_tgt, m_nt.2) m_nt.1 with
-    | Some expr_list => Some (module_graph_vertex_set_p.add (v_tgt, m_nt.2)    (Eref ref_src :: expr_list) m_nt.1, (m_nt.2 + 1)%num)
-    | None =>           Some (module_graph_vertex_set_p.add (v_tgt, m_nt.2) [:: Eref ref_src]              m_nt.1, (m_nt.2 + 1)%num)
-    end
-| Gtyp _ => Some (m_nt.1, (m_nt.2 + 1)%num)
-| Atyp t' _ => tmap_add_passive_connect m_nt v_tgt (Esubindex ref_src 0) t'
-| Btyp ff => tmap_add_passive_connect_fields m_nt v_tgt ref_src ff
-end
-with tmap_add_passive_connect_fields (m_nt : var2exprsmap * N) (v_tgt : VarOrder.t) (ref_src : HiFP.href) (ff : ffield) : option (var2exprsmap * N) :=
-match ff with
-| Fnil => Some m_nt
-| Fflips v Nflip   t ff' =>
-    match tmap_add_passive_connect m_nt v_tgt (Esubfield ref_src v) t with
-    | Some m_nt' => tmap_add_passive_connect_fields m_nt' v_tgt ref_src ff'
-    | None => None
-    end
-| Fflips v Flipped t ff' => None
 end.
 
 Fixpoint split_expr (ref_src : HiFP.href) (t : ftype) : option (seq HiFP.href) :=
@@ -553,37 +448,6 @@ with split_expr_non_passive_f (ref_src : HiFP.href) (ff : ffield) (fl : bool) : 
     end
   end.
 
-Fixpoint tmap_add_expr_connect (m_nt : var2exprsmap * N) (v_tgt : VarOrder.t) (expr_src : HiFP.hfexpr) (t : ftype) : option var2exprsmap :=
-(* add connections for all ground-type entries of ref_tgt <= expr_src.
-   This works for InferWidths, so for arrays it only adds one connection, not one connection per entry.
-   m_n is a pair: a var2exprsmap to which connections are added
-                  a natural number that indicates which index of ref_tgt is to be connected
-   v_tgt is the base variable name.
-   ref_tgt is the href that corresponds to (v_tgt, m_nt.2).
-   The return value is the updated var2exprsmap. *)
-match t, expr_src with
-| Gtyp (Fuint_implicit _), expr
-| Gtyp (Fsint_implicit _), expr =>
-    match module_graph_vertex_set_p.find (v_tgt, m_nt.2) m_nt.1 with
-    | Some expr_list => Some (module_graph_vertex_set_p.add (v_tgt, m_nt.2)    (expr_src :: expr_list) m_nt.1)
-    | None =>           Some (module_graph_vertex_set_p.add (v_tgt, m_nt.2) [:: expr_src]              m_nt.1)
-    end
-| Gtyp _, _ => Some m_nt.1
-(* In Emux and Evalidif (below) the condition is not important for width inference. So ignore it. *)
-| t, Emux _ e1 e2 =>
-    match tmap_add_expr_connect m_nt v_tgt e1 t with
-    | Some m' => tmap_add_expr_connect (m', m_nt.2) v_tgt e2 t
-    | None => None
-    end
-| t, Evalidif _ e => tmap_add_expr_connect m_nt v_tgt e t
-| t, Eref ref =>
-    match tmap_add_passive_connect m_nt v_tgt ref t with
-    | Some (m', _) => Some m'
-    | None => None
-    end
-| _, _ => None
-end.
-
 Fixpoint combine_mux_expr (c : HiFP.hfexpr) (el1 el2 : seq HiFP.hfexpr) : option (seq HiFP.hfexpr) :=
   match el1, el2 with
   | nil, nil => Some nil
@@ -614,9 +478,10 @@ Definition connect_fgtyp_compatible (t_tgt t_src : fgtyp) : bool :=
 Fixpoint check_connect_fgtyp_compatible (t_tgt t_src : ftype) (n : nat) : bool :=
   match n with
   | 0 => true
-  | S m => match ft_find_sub t_tgt (N.of_nat m), ft_find_sub t_src (N.of_nat m) with
-          | Some gt_tgt, Some gt_src => connect_fgtyp_compatible gt_tgt gt_src && check_connect_fgtyp_compatible t_tgt t_src m
-          | _,_ => false
+  | S m => match ft_check_flip t_tgt (N.of_nat m) false, ft_find_sub t_tgt (N.of_nat m), ft_find_sub t_src (N.of_nat m) with
+          | Some false, Some gt_tgt, Some gt_src => connect_fgtyp_compatible gt_tgt gt_src && check_connect_fgtyp_compatible t_tgt t_src m
+          | _,None,None => true
+          | _,_,_ => false
           end
   end.
 
@@ -626,6 +491,7 @@ Fixpoint check_connect_non_passive_fgtyp (t_tgt t_src : ftype) (n : nat) : bool 
   | S m => match ft_check_flip t_tgt (N.of_nat m) false, ft_find_sub t_tgt (N.of_nat m), ft_find_sub t_src (N.of_nat m) with
           | Some false, Some gt_tgt, Some gt_src => connect_fgtyp_compatible gt_tgt gt_src && check_connect_non_passive_fgtyp t_tgt t_src m
           | Some true, Some gt_tgt, Some gt_src => connect_fgtyp_compatible gt_src gt_tgt && check_connect_non_passive_fgtyp t_tgt t_src m
+          | _,None,None => true
           | _,_,_ => false
           end
   end.
@@ -635,34 +501,6 @@ Definition connect_non_passive_type (t_tgt : ftype) (t_src : ftype) : Prop :=
 
 Definition connect_type_compatible (t_tgt t_src : ftype) : bool :=
   ftype_equiv t_tgt t_src && check_connect_fgtyp_compatible t_tgt t_src (tmap_type_size t_tgt).
-
-(*match list_gtyp t_tgt, list_gtyp t_src with
-  | nil, nil => true
-  | hd1 :: tl1, 
-match t_tgt, t_src with
-| Gtyp (Fuint _), Gtyp (Fuint _)
-| Gtyp (Fuint _), Gtyp (Fuint_implicit _)
-| Gtyp (Fuint_implicit _), Gtyp (Fuint _)
-| Gtyp (Fuint_implicit _), Gtyp (Fuint_implicit _)
-| Gtyp (Fsint _), Gtyp (Fsint _)
-| Gtyp (Fsint _), Gtyp (Fsint_implicit _)
-| Gtyp (Fsint_implicit _), Gtyp (Fsint _)
-| Gtyp (Fsint_implicit _), Gtyp (Fsint_implicit _)
-| Gtyp Fclock, Gtyp Fclock
-| Gtyp Freset, Gtyp Freset
-| Gtyp Fasyncreset, Gtyp Fasyncreset => true
-| Atyp t_tgt' n_tgt, Atyp t_src' n_src => (n_tgt == n_src) && connect_type_compatible t_tgt' t_src'
-| Btyp ff_tgt, Btyp ff_src => connect_type_compatible_fields ff_tgt ff_src
-| _, _ => false
-end
-with connect_type_compatible_fields (ff_tgt ff_src : ffield) : bool :=
-match ff_tgt, ff_src with
-| Fnil, Fnil => true
-| Fflips v_tgt f_tgt t_tgt ff_tgt', Fflips v_src f_src t_src ff_src' =>
-    (v_tgt == v_src) && (fflip_eqn f_tgt f_src) && connect_type_compatible t_tgt t_src && connect_type_compatible_fields ff_tgt' ff_src'
-| _, _ => false
-end. (* should be none flip *)
-*)
 
 Fixpoint add_expr_connect (v : ProdVarOrder.t) (el : seq HiFP.hfexpr) (var2exprs : var2exprsmap) : var2exprsmap :=
   match el with
@@ -1159,61 +997,154 @@ match F with
                       end
   end.
 
-(*Definition connect_non_passive_gt (gt_tgt : fgtyp) (gt_src : fgtyp) : Prop :=
-  match gt_tgt, gt_src with
-      | Fuint _, Fuint _
-      | Fuint _, Fuint_implicit _
-      | Fsint _, Fsint _
-      | Fsint _, Fsint_implicit _
-      | Fclock, Fclock
-      | Freset, Freset
-      | Fasyncreset, Fasyncreset => True
-      | Fuint_implicit wt, Fuint ws
-      | Fuint_implicit wt, Fuint_implicit ws
-      | Fsint_implicit wt, Fsint ws
-      | Fsint_implicit wt, Fsint_implicit ws => wt >= ws
-      | _, _ => False
-      end.
+Lemma num_ref_eq : forall checkt nt0, ftype_equiv checkt nt0 -> tmap_type_size checkt = tmap_type_size nt0
+with num_ref_eq_f : forall checkf nf0, fbtyp_equiv checkf nf0 -> tmap_type_size_fields checkf = tmap_type_size_fields nf0.
+Proof.
+  clear num_ref_eq.
+  elim.
+  intro gt.
+  elim.
+  intros gt0 Heq.
+  simpl; done.
+  intros; simpl in H0; discriminate.
+  intros; simpl in H; discriminate.
 
-Fixpoint connect_non_passive_type (ft_tgt : ftype) (ft_src : ftype) : Prop :=
-  match ft_tgt, ft_src with
-   | Gtyp gt_tgt, Gtyp gt_src => connect_non_passive_gt gt_tgt gt_src
-   | Atyp elt_tgt n1, Atyp elt_src n2 => n1 = n2 /\ connect_non_passive_type elt_tgt elt_src
-   | Btyp ft, Btyp fs => connect_non_passive_type_fields ft fs 
-   | _, _ => False
-   end
-with connect_non_passive_type_fields (ft_tgt : ffield) (ft_src : ffield) : Prop :=
-  match ft_tgt, ft_src with
-   | Fnil, Fnil => True
-   | Fflips v1 Nflip gtt ft, Fflips v2 Nflip gts fs => v1 = v2 /\
-         connect_non_passive_type gtt gts /\
-         connect_non_passive_type_fields ft fs 
-   | Fflips v1 Flipped gtt ft, Fflips v2 Flipped gts fs => v1 = v2 /\
-         connect_non_passive_type_flipped gts gtt /\
-         connect_non_passive_type_fields ft fs
-   | _, _ => False
-   end
-with connect_non_passive_type_flipped (ft_tgt : ftype) (ft_src : ftype) : Prop :=
-   (* The code in this predicate is the same as in connect_non_passive. *)
-   match ft_tgt, ft_src with
-   | Gtyp gt_tgt, Gtyp gt_src => connect_non_passive_gt gt_tgt gt_src
-   | Atyp elt_tgt n1, Atyp elt_src n2 => n1 = n2 /\ connect_non_passive_type_flipped elt_tgt elt_src
-   | Btyp ft, Btyp fs => connect_non_passive_type_fields_flipped ft fs 
-   | _, _ => False
-   end
-with connect_non_passive_type_fields_flipped (ft_tgt : ffield) (ft_src : ffield) : Prop :=
-   (* The code in this predicate is the same as in connect_non_passive_fields. *)
-   match ft_tgt, ft_src with
-   | Fnil, Fnil => True
-   | Fflips v1 Nflip gtt ft, Fflips v2 Nflip gts fs => v1 = v2 /\
-         connect_non_passive_type_flipped gtt gts /\
-         connect_non_passive_type_fields_flipped ft fs 
-   | Fflips v1 Flipped gtt ft, Fflips v2 Flipped gts fs => v1 = v2 /\
-         connect_non_passive_type gts gtt /\
-         connect_non_passive_type_fields_flipped ft fs
-   | _, _ => False
-   end.
-*)
+  intros f H n.
+  elim.
+  intros; simpl in H0; discriminate.
+  intros f0 H' n0 Heq; clear H'.
+  simpl; simpl in Heq.
+  move /andP : Heq => [_ Heq].
+  apply H in Heq; rewrite Heq; done.
+  intros; simpl in H; discriminate.
+
+  intro f. 
+  elim.
+  intros; simpl in H; discriminate.
+  intros; simpl in H; discriminate.
+  intro f0.
+  simpl; intro Heq; apply num_ref_eq_f in Heq.
+  rewrite Heq; done.
+
+  clear num_ref_eq_f.
+  elim.
+  intros.
+  simpl in H.
+  case Hnf0 : nf0; rewrite Hnf0 in H; try discriminate; try done.
+  intros v fl ft ff Heq.
+  elim.
+  intros.
+  simpl in H. 
+  case Hfl : fl; rewrite Hfl in H; discriminate.
+  intros v0 fl0 ft0 ff0 H' Heq0; clear H'.
+  simpl.
+  simpl in Heq0.
+  case Hfl : fl; rewrite Hfl in Heq0.
+  case Hfl0 : fl0; rewrite Hfl0 in Heq0; try discriminate.
+  move /andP : Heq0 => [Heq0 Heq1].
+  move /andP : Heq0 => [_ Heq2].
+  apply num_ref_eq in Heq2.
+  apply Heq in Heq1.
+  rewrite Heq1 Heq2; done.
+  case Hfl0 : fl0; rewrite Hfl0 in Heq0; try discriminate.
+  move /andP : Heq0 => [Heq0 Heq1].
+  move /andP : Heq0 => [_ Heq2].
+  apply num_ref_eq in Heq2.
+  apply Heq in Heq1.
+  rewrite Heq1 Heq2; done.
+Qed.
+
+Lemma ft_set_sub_eq : forall checkt nt' nt0 n init, ft_find_sub checkt n = Some init -> fgtyp_equiv init nt' -> ft_set_sub checkt nt' n = Some nt0 -> ftype_equiv checkt nt0
+with ft_set_sub_eq_f : forall checkf nf' nf0 n init, ft_find_ff checkf n = Some init -> fgtyp_equiv init nf' -> ft_set_sub_f checkf nf' n = Some nf0 -> fbtyp_equiv checkf nf0.
+Proof.
+  clear ft_set_sub_eq.
+  elim.
+  intros f nt nt0 n init Hfind Heq Hset.
+  simpl in Hfind; simpl in Hset.
+  case Ha : (n == 0%num); rewrite Ha in Hfind Hset; try discriminate.
+  inversion Hfind; clear Hfind H0.
+  inversion Hset; clear Hset.
+  simpl; done.
+  
+  (* set aggt *)
+  intros f H n.
+  intros nt nt0 cnt init Hfind Heq Hset.
+  simpl in Hset.
+  simpl in Hfind.
+  case Hset' : (ft_set_sub f nt cnt) => [natyp|]; rewrite Hset' in Hset; try discriminate.
+  inversion Hset; clear Hset H1.
+  simpl.
+  apply rwP with (P := (n == n) /\ ftype_equiv f natyp).
+  apply andP.
+  split; try done.
+  move : Hfind Heq Hset'.
+  apply H.
+
+  (* set btyp *)
+  intros f nt nt0 cnt init Hfind Heq Hset.
+  simpl in Hfind.
+  simpl in Hset.
+  case Ha : (tmap_type_size_fields f <= cnt); rewrite Ha in Hfind Hset; try discriminate.
+  case Hset' : (ft_set_sub_f f nt cnt) => [newf|]; rewrite Hset' in Hset; try discriminate.
+  inversion Hset; clear Hset.
+  simpl.
+  move : Hfind Heq Hset'.
+  apply ft_set_sub_eq_f.
+
+  (* field *)
+  clear ft_set_sub_eq_f.
+  induction checkf.
+  intros.
+  simpl in H; discriminate.
+  intros nt nf0 cnt init Hfind Heq Hset.
+  simpl in Hfind.
+  simpl in Hset.
+  case Ha : (N.of_nat (tmap_type_size f0) <= cnt); rewrite Ha in Hfind Hset.
+  case Hset' : (ft_set_sub_f checkf nt (cnt - N.of_nat (tmap_type_size f0))) => [newf|]; rewrite Hset' in Hset; try discriminate.
+  inversion Hset; clear Hset.
+  simpl.
+  case Hf : f.
+  apply rwP with (P := (v == v) && ftype_equiv f0 f0 /\ fbtyp_equiv checkf newf).
+  apply andP.
+  split; try done.
+  apply rwP with (P := (v == v) /\ ftype_equiv f0 f0).
+  apply andP.
+  split; try done.
+  admit.
+  move : Hfind Heq Hset'.
+  apply IHcheckf.
+  apply rwP with (P := (v == v) && ftype_equiv f0 f0 /\ fbtyp_equiv checkf newf).
+  apply andP.
+  split; try done.
+  apply rwP with (P := (v == v) /\ ftype_equiv f0 f0).
+  apply andP.
+  split; try done.
+  admit.
+  move : Hfind Heq Hset'.
+  apply IHcheckf.
+  case Hset' : (ft_set_sub f0 nt cnt) => [newt'|]; rewrite Hset' in Hset; try discriminate.
+  inversion Hset; clear Hset.
+  simpl.
+  case Hf : f.
+  apply rwP with (P := (v == v) && ftype_equiv f0 newt' /\ fbtyp_equiv checkf checkf).
+  apply andP.
+  split; try done.
+  apply rwP with (P := (v == v) /\ ftype_equiv f0 newt').
+  apply andP.
+  split; try done.
+  move : Hfind Heq Hset'.
+  apply ft_set_sub_eq.
+  admit.
+  apply rwP with (P := (v == v) && ftype_equiv f0 newt' /\ fbtyp_equiv checkf checkf).
+  apply andP.
+  split; try done.
+  apply rwP with (P := (v == v) /\ ftype_equiv f0 newt').
+  apply andP.
+  split; try done.
+  move : Hfind Heq Hset'.
+  apply ft_set_sub_eq.
+  admit.
+Admitted.
 
 Lemma set_find_sub : forall checkt nt nt0 n, ft_set_sub checkt nt n = Some nt0 -> ftype_equiv checkt nt0 -> ft_find_sub nt0 n = Some nt
 with set_find_sub_f : forall checkf nf nf0 n, ft_set_sub_f checkf nf n = Some nf0 -> fbtyp_equiv checkf nf0 -> ft_find_ff nf0 n = Some nf.
@@ -1245,134 +1176,387 @@ Proof.
   case Hset' : (ft_set_sub_f f nt n) => [newf|]; rewrite Hset' in Hset; try discriminate.
   inversion Hset; clear Hset.
   simpl.
-  assert (tmap_type_size_fields newf = tmap_type_size_fields f).
-  admit.
-  rewrite H; clear H; rewrite Ha.
+  assert (tmap_type_size_fields f = tmap_type_size_fields newf).
+  apply num_ref_eq_f.
+  rewrite -H0 in Heq; simpl in Heq; done.
+  rewrite -H; clear H; rewrite Ha.
   rewrite -H0 in Heq; simpl in Heq.
   apply set_find_sub_f with (checkf := f); try done.
 
-  (*clear set_find_sub_f.
+  clear set_find_sub_f.
   intros checkf.
   induction checkf.
-  intros nf a nf0 n Hset Heq.
+  intros nf nf0 n Hset Heq.
   simpl in Hset; discriminate.
 
-  intros nf a hf0 n Hset Heq.
+  intros nf hf0 n Hset Heq.
   simpl in Hset.
-  case Hf : f; rewrite Hf in Hset; try discriminate.
-  case Ha : (a.2 == (n + 1)%num); rewrite Ha in Hset.
+  case Ha : (N.of_nat (tmap_type_size f0) <= n); rewrite Ha in Hset.
+  case Hset' : (ft_set_sub_f checkf nf (n - N.of_nat (tmap_type_size f0))) => [newf|]; rewrite Hset' in Hset; try discriminate.
   inversion Hset; clear Hset.
-  simpl; rewrite Ha; done.
-  case Ha' : ((n + N.of_nat (num_ref f0))%num < a.2); rewrite Ha' in Hset.
-  case Hset' : (ft_set_sub_f a checkf nf (n + N.of_nat (num_ref f0))) => [newf|]; rewrite Hset' in Hset; try discriminate.
-  inversion Hset; clear Hset.
-  apply IHcheckf in Hset'.
-  simpl; rewrite Ha Ha'; done.
-  rewrite -H0 in Heq.
-  simpl in Heq; rewrite Hf in Heq.
-  move /andP : Heq => [_ Heq]; done. 
-
-  case Hset' : (ft_set_sub a f0 nf (n+1)) => [newt'|]; rewrite Hset' in Hset; try discriminate.
-  inversion Hset; clear Hset.
-  assert ((num_ref f0) = (num_ref newt')).
+  assert (fbtyp_equiv checkf newf).
   rewrite -H0 in Heq.
   simpl in Heq.
-  rewrite Hf in Heq.
+  case Hf : f; rewrite Hf in Heq.
+  move /andP : Heq => [_ Heq]; done.
+  move /andP : Heq => [_ Heq]; done.
+  apply IHcheckf in Hset'; try done.
+  rewrite -Hset'.
+  simpl; rewrite Ha; done.
+
+  case Hset' : (ft_set_sub f0 nf n) => [newt'|]; rewrite Hset' in Hset; try discriminate.
+  inversion Hset; clear Hset.
+  simpl. 
+  assert ((tmap_type_size f0) = (tmap_type_size newt')).
+  rewrite -H0 in Heq.
+  simpl in Heq.
+  case Hf : f; rewrite Hf in Heq.
   move /andP : Heq => [Heq _].
   move /andP : Heq => [_ Heq].
   apply num_ref_eq; done.
-  rewrite H in Ha'; clear H.
-  simpl; rewrite Ha Ha'.
-  apply set_find_sub with (checkt := f0); try done.
-  rewrite -H0 in Heq.
-  simpl in Heq; rewrite Hf in Heq.
   move /andP : Heq => [Heq _].
   move /andP : Heq => [_ Heq].
-  done.*)
-Admitted.
+  apply num_ref_eq; done.
+  rewrite H in Ha; clear H.
+  simpl; rewrite Ha.
+  apply set_find_sub with (checkt := f0); try done.
+  rewrite -H0 in Heq.
+  simpl in Heq.
+  case Hf : f; rewrite Hf in Heq.
+  move /andP : Heq => [Heq _].
+  move /andP : Heq => [_ Heq]; done.
+  move /andP : Heq => [Heq _].
+  move /andP : Heq => [_ Heq]; done.
+Qed.
 
-Lemma ft_set_sub_eq : forall checkt nt' nt0 n init, ft_find_sub checkt n = Some init -> fgtyp_equiv init nt' -> ft_set_sub checkt nt' n = Some nt0 -> ftype_equiv checkt nt0
-with ft_set_sub_eq_f : forall checkf nf' nf0 n init, ft_find_ff checkf n = Some init -> fgtyp_equiv init nf' -> ft_set_sub_f checkf nf' n = Some nf0 -> fbtyp_equiv checkf nf0.
+Lemma infer_compatible : forall te otype nt, max_fgtyp te otype = Some nt -> connect_fgtyp_compatible nt otype /\ connect_fgtyp_compatible nt te.
 Proof.
-(* in InferWidths.v *)
+  intros.
+  (* ground match ground *)
+  case Hgt : te => [w'|w'|w'|w'|||]; rewrite Hgt in H.
+  (* te = Gtyp (uint w') *)
+  - case Hogt : otype => [ow'|ow'|ow'|ow'|||]; rewrite Hogt in H; simpl in H; try discriminate.
+    (* otype = Gtyp (uint ow') *)
+    inversion H; clear H. 
+    rewrite /connect_fgtyp_compatible.
+    simpl.
+    rewrite Nat.max_comm.
+    split.
+    apply rwP with (P := (ow' <= Nat.max ow' w') /\ true).
+    apply andP.
+    split; try done. 
+    (* rewrite <- Nat.le_max_l. *)
+    admit.
+    admit.
+  - case Hogt : otype => [ow'|ow'|ow'|ow'|||]; rewrite Hogt in H; simpl in H; try discriminate.
+    (* otype = Gtyp (uint ow') *)
+    inversion H; clear H. 
+    rewrite /connect_fgtyp_compatible.
+    simpl.
+    rewrite Nat.max_comm.
+    (*specialize Nat.le_max_l with (n := w') (m := ow').*)
+    admit.
+  - case Hogt : otype => [ow'|ow'|ow'|ow'|||]; rewrite Hogt in H; simpl in H; try discriminate.
+    (* otype = Gtyp (uint ow') *)
+    inversion H; clear H. 
+    rewrite /connect_fgtyp_compatible.
+    simpl.
+    rewrite Nat.max_comm.
+    (*specialize Nat.le_max_l with (n := w') (m := ow').*)
+    admit.
+  - case Hogt : otype => [ow'|ow'|ow'|ow'|||]; rewrite Hogt in H; simpl in H; try discriminate.
+    (* otype = Gtyp (uint ow') *)
+    inversion H; clear H. 
+    rewrite /connect_fgtyp_compatible.
+    simpl.
+    rewrite Nat.max_comm.
+    (*specialize Nat.le_max_l with (n := w') (m := ow').*)
+    admit.
+  - case Hogt : otype => [ow'|ow'|ow'|ow'|||]; rewrite Hogt in H; simpl in H; try discriminate.
+  - case Hogt : otype => [ow'|ow'|ow'|ow'|||]; rewrite Hogt in H; simpl in H; try discriminate.
+  - case Hogt : otype => [ow'|ow'|ow'|ow'|||]; rewrite Hogt in H; simpl in H; try discriminate.
 Admitted.
 
-Lemma max_compatible : forall el tmap otype nt eftl, fil_ftlist [seq type_of_hfexpr e tmap | e <- el] = Some eftl -> max_ftlist eftl otype = Some nt -> forall expr exprtype, expr \in el -> type_of_hfexpr expr tmap = Some exprtype -> connect_type_compatible (Gtyp nt) exprtype.
+Lemma fgtyp_equiv_dlvr : forall t1 t2 t3, fgtyp_equiv t1 t2 -> fgtyp_equiv t2 t3 -> fgtyp_equiv t1 t3.
+Proof.
+  intros.
+  case Ht1 : t1; case Ht2 : t2; case Ht3 : t3; rewrite Ht1 Ht2 in H; rewrite Ht2 Ht3 in H0; simpl in H; simpl in H0; simpl; try done; try discriminate.
+Qed.
+
+Lemma ftype_equiv_dlvr : forall t1 t2 t3, ftype_equiv t1 t2 -> ftype_equiv t2 t3 -> ftype_equiv t1 t3
+with ftype_equiv_dlvr_f : forall t1 t2 t3, fbtyp_equiv t1 t2 -> fbtyp_equiv t2 t3 -> fbtyp_equiv t1 t3.
+Proof.
+  elim.
+  intros gt1 t2 t3 H H0.
+  case Ht2 : t2 => [gt2|atyp2 n2|btyp2]; rewrite Ht2 in H H0; simpl in H; try discriminate.
+  case Ht3 : t3 => [gt3|atyp3 n3|btyp3]; rewrite Ht3 in H H0; simpl in H0; simpl; try done; try discriminate.
+  move : H H0; apply fgtyp_equiv_dlvr.
+
+  intros atyp1 IH n1 t2 t3 H H0.
+  case Ht2 : t2 => [gt2|atyp2 n2|btyp2]; rewrite Ht2 in H H0; simpl in H; try discriminate.
+  case Ht3 : t3 => [gt3|atyp3 n3|btyp3]; rewrite Ht3 in H H0; simpl in H0; simpl; try done; try discriminate.
+  move /andP : H => [H1 H].
+  move /andP : H0 => [H2 H0].
+  move /eqP : H1 => H1.
+  move /eqP : H2 => H2.
+  apply rwP with (P := (n1 == n3) /\ ftype_equiv atyp1 atyp3).
+  apply andP.
+  split.
+  rewrite H1 -H2; try done.
+  move : H H0; apply IH.
+
+  intros btyp t2 t3 H H0.
+  case Ht2 : t2 => [gt2|atyp2 n2|btyp2]; rewrite Ht2 in H H0; simpl in H; try discriminate.
+  case Ht3 : t3 => [gt3|atyp3 n3|btyp3]; rewrite Ht3 in H H0; simpl in H0; simpl; try done; try discriminate.
+  move : H H0; apply ftype_equiv_dlvr_f.
+
+  elim.
+  intros t2 t3 H H0.
+  case Ht2 : t2 => [|v2 fl2 ft2 f2]; rewrite Ht2 in H H0; simpl in H; try discriminate.
+  case Ht3 : t3 => [|v3 fl3 ft3 f3]; rewrite Ht3 in H0; simpl in H0; try discriminate.
+  simpl; done.
+  intros v1 fl1 ft1 f1 IH t2 t3 H H0.
+  case Ht2 : t2 => [|v2 fl2 ft2 f2]; rewrite Ht2 in H H0; simpl in H; case Hf1 : fl1; rewrite Hf1 in H; try discriminate.
+  case Hf2 : fl2; rewrite Hf2 in H; try discriminate.
+  case Ht3 : t3 => [|v3 fl3 ft3 f3]; rewrite Ht3 Hf2 in H0; simpl in H0; try discriminate.
+  case Hf3 : fl3; rewrite Hf3 in H0; try discriminate.
+  simpl.
+  move /andP : H => [H H1].
+  move /andP : H => [H H']. 
+  move /andP : H0 => [H0 H2].
+  move /andP : H0 => [H0 H3].
+  move /eqP : H => H.
+  move /eqP : H0 => H0.
+  apply rwP with (P := (v1 == v3) && ftype_equiv ft1 ft3 /\ fbtyp_equiv f1 f3).
+  apply andP.
+  split.
+  apply rwP with (P := (v1 == v3) /\ ftype_equiv ft1 ft3).
+  apply andP.
+  split.
+  rewrite H -H0; done.
+  move : H' H3; apply ftype_equiv_dlvr.
+  move : H1 H2; apply IH.
+  case Hf2 : fl2; rewrite Hf2 in H; try discriminate.
+  case Ht3 : t3 => [|v3 fl3 ft3 f3]; rewrite Ht3 Hf2 in H0; simpl in H0; try discriminate.
+  case Hf3 : fl3; rewrite Hf3 in H0; try discriminate.
+  simpl.
+  move /andP : H => [H H1].
+  move /andP : H => [H H']. 
+  move /andP : H0 => [H0 H2].
+  move /andP : H0 => [H0 H3].
+  move /eqP : H => H.
+  move /eqP : H0 => H0.
+  apply rwP with (P := (v1 == v3) && ftype_equiv ft1 ft3 /\ fbtyp_equiv f1 f3).
+  apply andP.
+  split.
+  apply rwP with (P := (v1 == v3) /\ ftype_equiv ft1 ft3).
+  apply andP.
+  split.
+  rewrite H -H0; done.
+  move : H' H3; apply ftype_equiv_dlvr.
+  move : H1 H2; apply IH.
+Qed.
+
+Lemma max_compatible' : forall gte gt tmax, max_fgtyp gte gt = Some tmax -> (sizeof_fgtyp gte <= sizeof_fgtyp tmax) && fgtyp_equiv tmax gte && fgtyp_equiv tmax gt && (sizeof_fgtyp gt <= sizeof_fgtyp tmax).
+Proof.
+  intros.
+  case Hgte : gte => [w'|w'|w'|w'|||]; rewrite Hgte in H.
+  (* gte = Gtyp (uint w') *)
+  - case Hgt : gt => [ow'|ow'|ow'|ow'|||]; rewrite Hgt in H; simpl in Hgt; simpl in H; try discriminate.
+    inversion H; clear H.
+    simpl.
+    rewrite Nat.max_comm.
+    admit. (* <= max *)
+  - case Hgt : gt => [ow'|ow'|ow'|ow'|||]; rewrite Hgt in H; simpl in Hgt; simpl in H; try discriminate.
+    inversion H; clear H.
+    simpl.
+    rewrite Nat.max_comm.
+    admit. (* <= max *)
+  - case Hgt : gt => [ow'|ow'|ow'|ow'|||]; rewrite Hgt in H; simpl in Hgt; simpl in H; try discriminate.
+    inversion H; clear H.
+    simpl.
+    rewrite Nat.max_comm.
+    admit. (* <= max *)
+  - case Hgt : gt => [ow'|ow'|ow'|ow'|||]; rewrite Hgt in H; simpl in Hgt; simpl in H; try discriminate.
+    inversion H; clear H.
+    simpl.
+    rewrite Nat.max_comm.
+    admit. (* <= max *)
+  - case Hgt : gt => [ow'|ow'|ow'|ow'|||]; rewrite Hgt in H; simpl in Hgt; simpl in H; try discriminate.
+  - case Hgt : gt => [ow'|ow'|ow'|ow'|||]; rewrite Hgt in H; simpl in Hgt; simpl in H; try discriminate.
+  - case Hgt : gt => [ow'|ow'|ow'|ow'|||]; rewrite Hgt in H; simpl in Hgt; simpl in H; try discriminate.
+Admitted.
+
+Lemma max_compatible : forall el tmap eftl initt tmax, fil_ftlist (map (fun e => type_of_hfexpr e tmap) el) = Some eftl -> forall expr gte, expr \in el -> type_of_hfexpr expr tmap = Some (Gtyp gte) -> max_ftlist eftl initt = Some tmax -> (sizeof_fgtyp gte <= sizeof_fgtyp tmax) && fgtyp_equiv tmax gte.
 Proof.
   elim.
   intros.
-  rewrite in_nil in H1; discriminate.
-  intros hd tl H tmap init nt eftl Hl Hmax.
-  simpl in Hl. 
-  (*case Hhd : (type_of_e hd tmap) => [nht|]; rewrite Hhd in Hl; try discriminate.
-  case Hl' : (fil_ftlist [seq type_of_e e tmap | e <- tl]) => [tl'|]; rewrite Hl' in Hl; try discriminate.
-  inversion Hl; clear Hl.
-  rewrite -H1 in Hmax.
-  simpl in Hmax.
-  case Hmax' : (max_ftlist tl' init) => [nt'|]; rewrite Hmax' in Hmax; try discriminate.
-
-  intros expr exprtype Hin Hexpr.
+  rewrite in_nil in H0; discriminate.
+  intros hd tl IH tmap eftl initt tmax Hfil expr gte Hin Hgte Hmax.
   rewrite in_cons in Hin.
   case Heq : (expr == hd).
+  (* case1 *)
   move /eqP : Heq => Heq.
-  rewrite Heq in Hexpr.
-  rewrite Hexpr in Hhd.
-  inversion Hhd; clear Hhd.
-  move : Hmax. (* infer_compatible *)
-  admit.
-  rewrite Heq in Hin; clear Heq. 
-  apply H with (tmap := tmap) (otype := init ) (nt := nt') (eftl := tl') (expr := expr) (exprtype := exprtype) in Hl'; try done.
-  apply connect_compatible_dlvr with (t1 := nt) (t2 := nt') (t3 := exprtype); try done.
-  move : Hmax.
-  apply infer_compatible.*)
-Admitted.
+  rewrite Heq in Hgte.
+  simpl in Hfil. 
+  rewrite Hgte in Hfil. 
+  case Hfil' : (fil_ftlist [seq type_of_hfexpr e tmap | e <- tl]) => [eftl'|]; rewrite Hfil' in Hfil; try discriminate.
+  inversion Hfil; clear Hfil.
+  rewrite -H0 in Hmax.
+  simpl in Hmax.
+  case Hmax' : (max_ftlist eftl' initt) => [tmax'|]; rewrite Hmax' in Hmax; try discriminate.
+  specialize max_compatible' with (gte := gte) (gt := tmax') (tmax := tmax); intro.
+  apply H in Hmax; clear H.
+  move /andP : Hmax => [H1 _].
+  move /andP : H1 => [H1 _]; done.
+  (* case2 *)
+  rewrite Heq in Hin.
+  rewrite orb_false_l in Hin; clear Heq.
+  simpl in Hfil.
+  case Hhd : (type_of_hfexpr hd tmap) => [t|]; rewrite Hhd in Hfil;  try discriminate.
+  case Hgt : t =>[gt||]; rewrite Hgt in Hfil; try discriminate.
+  case Hfil' : (fil_ftlist [seq type_of_hfexpr e tmap | e <- tl]) => [eftl'|]; rewrite Hfil' in Hfil; try discriminate.
+  inversion Hfil; clear Hfil.
+  rewrite -H0 in Hmax.
+  simpl in Hmax.
+  case Hmax' : (max_ftlist eftl' initt) => [tmax'|]; rewrite Hmax' in Hmax; try discriminate.
+  apply IH with (initt := initt) (tmax := tmax') (expr := expr) (gte := gte) in Hfil'; try done.
+  move /andP : Hfil' => [H1 H2].
+  apply rwP with (P := (sizeof_fgtyp gte <= sizeof_fgtyp tmax) /\ fgtyp_equiv tmax gte).
+  apply andP.
+  split.
+  specialize max_compatible' with (gte := gt) (gt := tmax') (tmax := tmax); intro H.
+  apply H in Hmax; clear H.
+  move /andP : Hmax => [_ H3].
+  move : H1 H3.
+  apply leq_trans.
+  specialize max_compatible' with (gte := gt) (gt := tmax') (tmax := tmax); intro H.
+  apply H in Hmax; clear H.
+  move /andP : Hmax => [Hmax _].
+  move /andP : Hmax => [_ H3].
+  move : H3 H2.
+  apply fgtyp_equiv_dlvr.
+Qed.
 
 Lemma inferwidths_a : forall a v expr_seq tmap tmap', InferWidth_fun v expr_seq tmap = Some tmap' -> 
-  if (a == v) then True 
-  else match CEP.find (fst a, N0) tmap, CEP.find (fst a, N0) tmap' with
+  if (a != v) then 
+  match CEP.find (fst a, N0) tmap, CEP.find (fst a, N0) tmap' with
         | Some ft, Some ft' => ft_find_sub ft (snd a) = ft_find_sub ft' (snd a)
         | _, _ => True
-        end.
+        end
+  else True.
 Proof.
-  (* 这个定理不对了
   intros.
-  case Heq : (a == v); try done.
-  case Heq' : ((a.1 == v.1) && (a.2 != v.2)).
-  move /andP : Heq' => [H0 H1]; clear Heq.
-  move /eqP : H0 => H0.
-  rewrite H0. 
+  case Heq : (a != v); try done.
+  case Ha : (CEP.find (a.1, 0%num) tmap) => [ft|]; try done.
+  case Ha' : (CEP.find (a.1, 0%num) tmap') => [ft'|]; try done.
+
   rewrite /InferWidth_fun in H.
-  case Hel : (fil_ftlist [seq type_of_e e tmap | e <- expr_seq]) => [eftl|]; rewrite Hel in H; try discriminate.
-  case Hfindv0 : (ft_find (v.1, 0%num) tmap) => [init|]; rewrite Hfindv0 in H; try discriminate.
-  case Hsub : (ft_find_sub v init 0) => [initt|]; rewrite Hsub in H; try discriminate.
-  case Hmax : (max_ftlist eftl initt) => [nt|]; rewrite Hmax in H; try discriminate.
-  case Hinfer : (InferWidth_ref v init nt) => [nt0|]; rewrite Hinfer in H; try discriminate.
+  case Hel : (fil_ftlist [seq type_of_hfexpr e tmap | e <- expr_seq]) => [eftl|]; rewrite Hel in H; try discriminate.
+  case Hfindv0 : (CEP.find (v.1, 0%num) tmap) => [init|]; rewrite Hfindv0 in H; try discriminate.
+  case Hsub : (ft_find_sub init v.2) => [initt|]; rewrite Hsub in H; try discriminate.
+  case Himpli : (not_implicit initt); rewrite Himpli in H.
+  (* case1 *)
   inversion H; clear H.
-  rewrite ft_find_add.
-  rewrite /InferWidth_ref in Hinfer.
-  rewrite Hsub in Hinfer.
-  case Hinfer' : (infer_implicit initt nt) => [newt|]; rewrite Hinfer' in Hinfer; try discriminate.
-  (* forall a v, a.1 = v.1 -> a.2 != v.2 -> ft_set_sub v init newt 0 = Some nt0 -> ft_set_sub v init newt 0 = Some nt0. *)
-  admit. (* inferref只改了v位置上的，故find_sub a应该相等 *)
-  assert (a.1 != v.1).
-  admit. (* 由Heq Heq'推出a.1!=v.1 *)
-  rewrite /InferWidth_fun in H.
-  case Hel : (fil_ftlist [seq type_of_e e tmap | e <- expr_seq]) => [eftl|]; rewrite Hel in H; try discriminate.
-  case Hfindv0 : (ft_find (v.1, 0%num) tmap) => [init|]; rewrite Hfindv0 in H; try discriminate.
-  case Hsub : (ft_find_sub v init 0) => [initt|]; rewrite Hsub in H; try discriminate.
+  rewrite H1 in Ha.
+  rewrite Ha in Ha'.
+  inversion Ha'; done.
+  (* case2 *)
   case Hmax : (max_ftlist eftl initt) => [nt|]; rewrite Hmax in H; try discriminate.
-  case Hinfer : (InferWidth_ref v init nt) => [nt0|]; rewrite Hinfer in H; try discriminate.
+  case Hinfer : (ft_set_sub init nt v.2) => [nt0|]; rewrite Hinfer in H; try discriminate.
   inversion H; clear H.
-  case Hfinda0 : (ft_find (a.1, 0%num) tmap) => [ft|]; try done.
-  (* find_add_not. forall a v nt tmap, ft_find a tmap = ft_find a (ft_add v nt tmap) *)
-  admit.  ft = ft' *)
+  rewrite -H1 in Ha'.
+  rewrite HiFP.PCELemmas.OP.P.F.add_neq_o in Ha'.
+  rewrite Ha' in Ha. 
+  inversion Ha; done.
 Admitted.
 
 Lemma inferwidths_ls : forall el a var2exprs tmap tmap' checkt checkt', InferWidths_fun el var2exprs tmap = Some tmap' -> 
-  ~(a \in el) -> CEP.find (fst a, N0) tmap' = Some checkt' -> CEP.find (fst a, N0) tmap = Some checkt -> ft_find_sub checkt (snd a) = ft_find_sub checkt' (snd a).
+  ~~(a \in el) -> CEP.find (fst a, N0) tmap' = Some checkt' -> CEP.find (fst a, N0) tmap = Some checkt -> ft_find_sub checkt (snd a) = ft_find_sub checkt' (snd a).
 Proof.
- (* 这个定理不对了 *)
-  
+  elim.
+  intros.
+  simpl in H. 
+  inversion H; clear H. 
+  rewrite H4 in H2.
+  rewrite H2 in H1.
+  inversion H1; done.
+  intros hd tl IH a var2exprs tmap tmap' checkt checkt' Hinfer Hin Hcheckt' Hcheckt.
+  rewrite in_cons in Hin.
+  rewrite negb_or in Hin.
+  move /andP : Hin => [H H1].
+  simpl in Hinfer.
+  case Hel : (module_graph_vertex_set_p.find hd var2exprs) => [el|]; rewrite Hel in Hinfer; try discriminate.
+  case Hinfer' : (InferWidth_fun hd el tmap) => [newtm|]; rewrite Hinfer' in Hinfer; try discriminate.
+  specialize inferwidths_a with (v := hd) (a := a) (expr_seq := el) (tmap := tmap) (tmap' := newtm); intro.
+  apply H0 in Hinfer'; clear H0.
+  rewrite H Hcheckt in Hinfer'.
+  case Hnewtm : (CEP.find (a.1, 0%num) newtm) => [newt|]; rewrite Hnewtm in Hinfer'.
+  apply IH with (a:= a) (checkt := newt) (checkt' := checkt') in Hinfer; try done.
+  rewrite Hinfer' -Hinfer; done.
+  admit. (* Hnewtm 不是None *)
+Admitted.
+
+Lemma max_ftlist_correct : forall eftl initt tmax, max_ftlist eftl initt = Some tmax -> (not_implicit initt = false -> not_implicit tmax = false) /\ fgtyp_equiv initt tmax.
+Proof.
+  elim.
+  intros.
+  split.
+  intros.
+  simpl in H. 
+  inversion H.
+  rewrite -H2; done.
+  simpl in H. 
+  inversion H.
+  admit.
+
+  intros hd tl H init nt Hl.
+  split.
+  intro Himpli.
+  simpl in Hl. 
+  case Htl : (max_ftlist tl init) => [nt'|]; rewrite Htl in Hl; try discriminate.
+  apply H in Htl; try done.
+  rewrite /max_fgtyp in Hl.
+  case Hhd : hd; rewrite Hhd in Hl; try discriminate.
+  case Hnt' : nt'; rewrite Hnt' in Hl Htl; try discriminate; inversion Hl; simpl; try done.
+  case Hnt' : nt'; rewrite Hnt' in Hl Htl; try discriminate; inversion Hl; simpl; try done.
+  case Hnt' : nt'; rewrite Hnt' in Hl Htl; try discriminate; inversion Hl; simpl; try done.
+  case Hnt' : nt'; rewrite Hnt' in Hl Htl; try discriminate; inversion Hl; simpl; try done.
+
+  simpl in Hl. 
+  case Htl : (max_ftlist tl init) => [nt'|]; rewrite Htl in Hl; try discriminate.
+  apply H in Htl; try done.
+  move : Htl => [_ Htl].
+  specialize max_compatible' with (gte := hd) (gt := nt') (tmax := nt); intro.
+  apply H0 in Hl; clear H0.
+  move /andP : Hl => [H1 _].
+  move /andP : H1 => [_ H1].
+  assert (fgtyp_equiv nt' nt).
+  admit.
+  move : Htl H0.
+  apply fgtyp_equiv_dlvr.
+Admitted.
+
+Lemma type_of_hfexpr_eq : forall (expr : HiFP.hfexpr) (pv : ProdVarOrder.t) (nt0 : ftype) (tmap : CEP.t ftype), type_of_hfexpr expr (CEP.add (pv.1, 0%num) nt0 tmap) = type_of_hfexpr expr tmap.
+Proof.
+  elim. 
+  - intros.
+    simpl; done.
+  - (*intros.
+    case Hu : u.
+    simpl.*)
+    admit.
+    admit.
+    admit.
+    admit.
+    admit.
+  - (* ref *)
+    intros ref pv nt0 tmap. 
+    simpl.
+    move : ref.
+    elim. 
+    intro ref.
+    rewrite /base_ref.
 Admitted.
 
 Lemma InferWidth_fun_correct : forall pv el tmap newtm, InferWidth_fun pv el tmap = Some newtm -> forall expr, expr \in el -> 
@@ -1418,10 +1602,364 @@ Proof.
   apply set_find_sub in Hset; try done.
   rewrite Hset in Hnt; clear Hset.
   inversion Hnt; clear Hnt.
-  rewrite -H0; clear H0.
-  apply max_compatible with (el := el) (tmap := tmap) (otype := initt) (eftl := eftl) (expr := expr); try done.
-  admit. (* 由于不成环，不影响expr的type，由Hte *)
-  admit. (* ft_set 的性质，由Hset *)
+  rewrite -H0.
+  rewrite /connect_type_compatible.
+  simpl.
+  case Hgte : te => [gte||]; rewrite Hgte in Heq; simpl in Heq; try discriminate.
+  apply rwP with (P := fgtyp_equiv tmax gte /\
+    match ft_find_sub (Gtyp gte) 0 with
+    | Some gt_src => connect_fgtyp_compatible tmax gt_src && true
+    | None => false
+    end).
+  apply andP. 
+  split.
+  rewrite -H0 in Heq; done.
+  simpl.
+  apply rwP with (P := connect_fgtyp_compatible tmax gte /\ true).
+  apply andP. 
+  split; try done.
+  rewrite /connect_fgtyp_compatible.
+  specialize max_ftlist_correct with (eftl := eftl) (initt := initt) (tmax := tmax); intro.
+  generalize Hmax.
+  apply H in Hmax; clear H.
+  move => Hmax'.
+  move : Hmax => [Hmax _].
+  apply Hmax in Himpli.
+  rewrite Himpli.
+  assert (type_of_hfexpr expr (CEP.add (pv.1, 0%num) nt0 tmap) = type_of_hfexpr expr tmap).
+  admit.
+  rewrite H in Hte; clear H.
+  rewrite Hgte in Hte.
+  apply max_compatible with (el := el) (tmap := tmap) (eftl := eftl) (initt := initt) (expr := expr); try done.
+  apply ft_set_sub_eq with (nt' := tmax) (n := pv.2) (init := initt); try done.
+  specialize max_ftlist_correct with (eftl := eftl) (initt := initt) (tmax := tmax); intro.
+  apply H in Hmax; clear H.
+  move : Hmax => [_ Hmax]; done.
+Admitted.
+
+Lemma ftype_eq_find_some : forall t1 t2 n te, ftype_equiv t1 t2 -> ft_find_sub t1 n = Some te -> 
+  exists b, ft_check_flip t1 n false = Some b /\ exists te', ft_find_sub t2 n = Some te'.
+Proof.
+Admitted.
+
+Lemma ftype_eq_check_flip : forall t1 t2 n, ftype_equiv t1 t2 -> ft_check_flip t1 n = ft_check_flip t2 n. 
+Proof.
+Admitted.
+
+
+Lemma check_connect_fgtyp_compatible4n ft te : forall n, (forall n0, n0 < n -> ft_check_flip ft (N.of_nat n0) false = Some false) -> (forall n0 gt gte, n0 < n -> ft_check_flip ft (N.of_nat n0) false = Some false -> ft_find_sub ft (N.of_nat n0) = Some gt -> ft_find_sub te (N.of_nat n0) = Some gte ->
+  connect_fgtyp_compatible gt gte) -> ftype_equiv ft te -> check_connect_fgtyp_compatible ft te n.
+Proof.
+  induction n. 
+  intros.
+  simpl; done.
+  intros Hnflip H Heq. 
+  simpl.
+  generalize Hnflip; specialize Hnflip with (n0 := n).
+  rewrite Hnflip; try done.
+  intro Hnflip'.
+  case Htgt : (ft_find_sub ft (N.of_nat n)) => [gt_tgt|].
+  case Hsrc : (ft_find_sub te (N.of_nat n)) => [gt_src|].
+  apply rwP with (P := connect_fgtyp_compatible gt_tgt gt_src /\ check_connect_fgtyp_compatible ft te n).
+  apply andP. 
+  split.
+  apply H with (n0 := n); try done.
+  apply Hnflip; try done.
+  apply IHn; try done.
+  intros.
+  apply Hnflip'.
+  rewrite -(addn1 n).
+  move : H0.
+  apply ltn_addr.
+  intros.
+  apply H with (n0 := n0); try done.
+  rewrite -(addn1 n).
+  move : H0.
+  apply ltn_addr.
+  apply ftype_eq_find_some with (t2 := te) in Htgt; try done.
+  destruct Htgt as [b [Hb [te' Htgt]]].
+  rewrite Htgt in Hsrc; discriminate.
+  case Hsrc : (ft_find_sub te (N.of_nat n)) => [te'|]; try done.
+  apply ftype_eq_find_some with (t2 := ft) in Hsrc; try done.
+  destruct Hsrc as [b [Hb [ft' Hsrc]]].
+  rewrite Htgt in Hsrc; discriminate.
+Admitted.
+
+Lemma check_connect_non_passive_fgtyp4n ft te : forall n, (forall n0 gt gte, n0 < n -> ft_find_sub ft (N.of_nat n0) = Some gt -> ft_find_sub te (N.of_nat n0) = Some gte ->
+        match ft_check_flip ft (N.of_nat n0) false with
+        | Some false => connect_fgtyp_compatible gt gte
+        | Some true => connect_fgtyp_compatible gte gt
+        | None => true
+        end) -> ftype_equiv ft te ->
+        check_connect_non_passive_fgtyp ft te n.
+Proof.
+  induction n. 
+  intros.
+  simpl; done.
+  intros H Heq. 
+  simpl.
+  case Hflip : (ft_check_flip ft (N.of_nat n) false) => [b|].
+  case Hb : b; rewrite Hb in Hflip.
+  (* case1 : flip *)
+  case Htgt : (ft_find_sub ft (N.of_nat n)) => [gt_tgt|].
+  case Hsrc : (ft_find_sub te (N.of_nat n)) => [gt_src|].
+  apply rwP with (P := connect_fgtyp_compatible gt_src gt_tgt /\ check_connect_non_passive_fgtyp ft te n).
+  apply andP. 
+  split.
+  specialize H with (n0 := n) (gt := gt_tgt) (gte := gt_src).
+  rewrite Hflip in H. 
+  apply H; try done.
+  apply IHn; try done.
+  intros.
+  case Hflip' : (ft_check_flip ft (N.of_nat n0) false) => [b0|]; try done.
+  apply H with (n0 := n0) (gt := gt) (gte := gte) in H1; try done.
+  rewrite Hflip' in H1; done.
+  rewrite -(addn1 n).
+  move : H0.
+  apply ltn_addr.
+  apply ftype_eq_find_some with (t2 := te) in Htgt; try done.
+  destruct Htgt as [b' [Hb' [te' Htgt]]].
+  rewrite Htgt in Hsrc; discriminate.
+  case Hsrc : (ft_find_sub te (N.of_nat n)) => [te'|]; try done.
+  apply ftype_eq_find_some with (t2 := ft) in Hsrc; try done.
+  destruct Hsrc as [b' [Hb' [ft' Hsrc]]].
+  rewrite Htgt in Hsrc; discriminate.
+  admit.
+  (* case2 : nflip *)
+  case Htgt : (ft_find_sub ft (N.of_nat n)) => [gt_tgt|].
+  case Hsrc : (ft_find_sub te (N.of_nat n)) => [gt_src|].
+  apply rwP with (P := connect_fgtyp_compatible gt_tgt gt_src /\ check_connect_non_passive_fgtyp ft te n).
+  apply andP. 
+  split.
+  specialize H with (n0 := n) (gt := gt_tgt) (gte := gt_src).
+  rewrite Hflip in H. 
+  apply H; try done.
+  apply IHn; try done.
+  intros.
+  case Hflip' : (ft_check_flip ft (N.of_nat n0) false) => [b0|]; try done.
+  apply H with (n0 := n0) (gt := gt) (gte := gte) in H1; try done.
+  rewrite Hflip' in H1; done.
+  rewrite -(addn1 n).
+  move : H0.
+  apply ltn_addr.
+  apply ftype_eq_find_some with (t2 := te) in Htgt; try done.
+  destruct Htgt as [b' [Hb' [te' Htgt]]].
+  rewrite Htgt in Hsrc; discriminate.
+  case Hsrc : (ft_find_sub te (N.of_nat n)) => [te'|]; try done.
+  apply ftype_eq_find_some with (t2 := ft) in Hsrc; try done.
+  destruct Hsrc as [b' [Hb' [ft' Hsrc]]].
+  rewrite Htgt in Hsrc; discriminate.
+  admit.
+  case Hsrc : (ft_find_sub te (N.of_nat n)) => [te'|]; try done.
+  apply ftype_eq_find_some with (t2 := ft) in Hsrc; try done.
+  destruct Hsrc as [b' [Hb' [ft' Hsrc]]].
+  apply ftype_eq_check_flip with (n := N.of_nat n) in Heq.
+  rewrite Heq in Hflip.
+  rewrite Hflip in Hb'; discriminate.
+  admit.
+  case Htgt : (ft_find_sub ft (N.of_nat n)) => [ft'|]; try done.
+  apply ftype_eq_find_some with (t2 := te) in Htgt; try done.
+  destruct Htgt as [b' [Hb' [te' Htgt]]].
+  rewrite Htgt in Hsrc; discriminate.
+Admitted.
+
+Lemma infer_cons_order : forall order1 order2 var2exprs tmap tmap' newtm, InferWidths_fun (order1 ++ order2) var2exprs tmap = Some newtm -> InferWidths_fun order1 var2exprs tmap = Some tmap' ->
+  InferWidths_fun order2 var2exprs tmap' = Some newtm.
+Proof.
+  elim. 
+  intros.
+  simpl in H0.
+  inversion H0; clear H0.
+  rewrite H2 in H.
+  simpl in H; done.
+  intros hd tl IH order2 var2exprs tmap tmap' newtm H H0.
+  simpl in H; simpl in H0.
+  case Hhd : (module_graph_vertex_set_p.find hd var2exprs) => [el|]; rewrite Hhd in H H0; try discriminate.
+  case Hinfer : (InferWidth_fun hd el tmap) => [tm|]; rewrite Hinfer in H H0; try discriminate.
+  move : H H0.
+  apply IH.
+Qed.
+
+Lemma find_mux_types_n : forall n t1 t2 t_expr tt1 tt2, mux_types t1 t2 = Some t_expr -> ft_find_sub t1 n = Some tt1 -> 
+  ft_find_sub t2 n = Some tt2 -> mux_gtyp tt1 tt2 = ft_find_sub t_expr n.
+Proof.
+  
+Admitted.
+
+Lemma combine_mux_expr_n : forall c el1 el2 rhs_expr_ls n e1 e2, combine_mux_expr c el1 el2 = Some rhs_expr_ls -> 
+  nth_error el1 n = Some e1 -> nth_error el2 n = Some e2 -> nth_error rhs_expr_ls n = Some (Emux c e1 e2).
+Proof.
+
+Admitted.
+
+Lemma split_expr_correct : forall s1 tmap t1 el1 e1 n gt, type_of_hfexpr s1 tmap = Some t1 -> split_expr_connect s1 t1 = Some el1 -> nth_error el1 n = Some e1 -> ft_find_sub t1 (N.of_nat n) = Some gt -> type_of_hfexpr e1 tmap = Some (Gtyp gt).
+Proof.
+Admitted.
+
+Lemma ftype_equiv_split_eq : forall s t1 t2, ftype_equiv t1 t2 -> split_expr_connect s t1 = split_expr_connect s t2.
+Proof.
+Admitted.
+
+Lemma mux_expr_type_equiv : forall c s1 s2 tmap te te1 te2, type_of_hfexpr (Emux c s1 s2) tmap = Some te -> type_of_hfexpr s1 tmap = Some te1 -> 
+  type_of_hfexpr s2 tmap = Some te2 -> ftype_equiv te te1 /\ ftype_equiv te te2.
+Proof.
+Admitted.
+
+Lemma split_expr_type_correct : (forall expr rhs_expr_ls t_expr newtm, type_of_hfexpr expr newtm = Some t_expr -> split_expr_connect expr t_expr = Some rhs_expr_ls ->  (* 这里可以加bool list用来判断flip *)
+  forall n, match ft_find_sub t_expr (N.of_nat n), List.nth_error rhs_expr_ls n with
+                        | Some gt, Some texpr => type_of_hfexpr texpr newtm = Some (Gtyp gt)
+                        | _, _ => true
+                        end).
+Proof.
+  elim.
+  intros.
+  simpl in H0.
+  inversion H0; clear H0.
+  move : n.
+  induction n as [|n]; simpl.
+  simpl in H. 
+  inversion H.
+  simpl; done.
+  simpl in H.
+  inversion H.
+  simpl; done.
+
+  admit.
+  admit.
+  admit.
+
+  (* mux case *)
+  intros c Hc s1 Hs1 s2 Hs2.
+  intros rhs_expr_ls t_expr tmap Hte Hsplit.
+  simpl in Hsplit.
+  case Hsplit1 : (split_expr_connect s1 t_expr) => [el1|]; rewrite Hsplit1 in Hsplit; try discriminate.
+  case Hsplit2 : (split_expr_connect s2 t_expr) => [el2|]; rewrite Hsplit2 in Hsplit; try discriminate.
+
+  generalize Hte.
+  simpl in Hte.
+  move => Hte'. 
+  case Hce : (type_of_hfexpr c tmap) => [f|]; rewrite Hce in Hte; try discriminate.
+  case Hcf : f => [cgt||]; rewrite Hcf in Hte; try discriminate.
+  case Hcgt : cgt => [w|w|w||||]; rewrite Hcgt in Hcf Hte; try discriminate.
+  case Hw : w => [|n0]; rewrite Hw in Hte; try discriminate.
+  case Hw' : n0; rewrite Hw' in Hte Hw; try discriminate.
+  rewrite Hw in Hcf; clear Hw Hw' Hcgt w n0 cgt.
+  case Hs1e : (type_of_hfexpr s1 tmap) => [t1|]; rewrite Hs1e in Hte; try discriminate.
+  case Hs2e : (type_of_hfexpr s2 tmap) => [t2|]; rewrite Hs2e in Hte; try discriminate.
+
+  intro n. 
+  case Hten : (ft_find_sub t_expr (N.of_nat n)) => [gte|]; try done.
+  case Hs1n : (ft_find_sub t1 (N.of_nat n)) => [tt1|].
+  case Hs2n : (ft_find_sub t2 (N.of_nat n)) => [tt2|].
+  apply find_mux_types_n with (n := N.of_nat n) (tt1 := tt1) (tt2 := tt2) in Hte; try done.
+  rewrite Hten in Hte; clear Hten.
+
+  assert (exists e1, nth_error el1 n = Some e1).
+  admit.
+  destruct H as [e1 He1].
+  assert (exists e2, nth_error el2 n = Some e2).
+  admit.
+  destruct H as [e2 He2].
+  apply combine_mux_expr_n with (n := n) (el1 := el1) (el2 := el2) (e1 := e1) (e2 := e2) in Hsplit; try done.
+  rewrite Hsplit.
+  simpl.
+  rewrite Hce Hcf.
+  case Hte1 : (type_of_hfexpr e1 tmap) => [te1|].
+  case Hte2 : (type_of_hfexpr e2 tmap) => [te2|].
+  generalize Hs1e.
+  apply split_expr_correct with (el1 := el1) (e1 := e1) (n := n) (gt := tt1) in Hs1e; try done.
+  rewrite Hs1e in Hte1; clear Hs1e.
+  move => Hs1e.
+  inversion Hte1; clear Hte1.
+  apply split_expr_correct with (el1 := el2) (e1 := e2) (n := n) (gt := tt2) in Hs2e; try done.
+  rewrite Hs2e in Hte2; clear Hs2e.
+  inversion Hte2; clear Hte2.
+  simpl; rewrite Hte; done.
+  specialize ftype_equiv_split_eq with (s := s2) (t1 := t_expr) (t2 := t2); intro.
+  rewrite H in Hsplit2.
+  done.
+  apply mux_expr_type_equiv with (c := c) (s1 := s1) (s2 := s2) (te := t_expr) (te1 := t1) (te2 := t2) in Hte'; try done.
+  move : Hte' => [_ Hte']; done.
+  specialize ftype_equiv_split_eq with (s := s1) (t1 := t_expr) (t2 := t1); intro.
+  rewrite H in Hsplit1.
+  done.
+  apply mux_expr_type_equiv with (c := c) (s1 := s1) (s2 := s2) (te := t_expr) (te1 := t1) (te2 := t2) in Hte'; try done.
+  move : Hte' => [Hte' _]; done.
+  admit. (* not None *)
+  admit. (* not None *)
+  admit. (* not None *)
+  admit. (* not None *)
+
+  admit. (* 与Fuint w的case完全一样 *)
+
+  admit. (* validif *)
+  admit. (* ref *)
+Admitted.
+
+(*Lemma add_non_passive2exprmap : forall lhsl rhsl v_tgt v_src var2exprs0 var2exprs refl bl refr br n, add_expr_connect_non_passive v_tgt v_src lhsl rhsl var2exprs0 = Some var2exprs ->
+  nth_error lhsl n = Some (refl, bl) -> nth_error rhsl n = Some (refr, br) -> match bl, br with
+  | true, true => match module_graph_vertex_set_p.find (v_src.1, N.add v_src.2 (N.of_nat n)) var2exprs with
+                | Some el => (Eref refl) \in el
+                | None => false
+                end
+  | false, false => match module_graph_vertex_set_p.find (v_tgt.1, N.add v_tgt.2 (N.of_nat n)) var2exprs with
+                | Some el => (Eref refr) \in el
+                | None => false
+                end
+  | _,_ => true
+  end.
+Proof.
+  elim.
+  admit.
+  intros hdl tll IH.
+  elim.
+  admit.
+  intros hdr tlr H; clear H.
+  specialize IH with (rhsl := tlr).
+  intros v_tgt v_src var2exprs0 var2exprs refl bl refr br.
+  simpl in Hadd.*)
+
+(* TBD!!重要 *)
+Lemma split_non_passive_correct : forall (ref_tgt ref_src : HiFP.href) (t_tgt t_src : ftype) (v_tgt v_src : ProdVarOrder.t) (tmap0 tmap : CEP.t ftype) (var2exprs0 var2exprs : var2exprsmap),
+  stmt_tmap (tmap0, var2exprs0) (Sfcnct ref_tgt (Eref ref_src)) = Some (tmap, var2exprs) ->
+  base_ref ref_tgt tmap0 = Some (v_tgt, t_tgt) -> base_ref ref_src tmap0 = Some (v_src, t_src) ->
+  match split_expr_non_passive ref_tgt t_tgt false, split_expr_non_passive ref_src t_src false with
+  | Some lhsl, Some rhsl => (forall n, n < length lhsl -> match List.nth_error lhsl n, List.nth_error rhsl n with
+                            | Some (_, false), Some (ref2, false) => match module_graph_vertex_set_p.find (v_tgt.1, N.add v_tgt.2 (N.of_nat n)) var2exprs with
+                                                          | Some el => (Eref ref2) \in el
+                                                          | None => false
+                                                          end
+                            | Some (ref1, true), Some (_, true) => match module_graph_vertex_set_p.find (v_src.1, N.add v_src.2 (N.of_nat n)) var2exprs with
+                                                          | Some el => (Eref ref1) \in el
+                                                          | None => false
+                                                          end
+                            | _,_ => false
+                            end)
+  | _, _ => false
+  end.
+Proof.
+  intros.
+  simpl in H.
+  rewrite H0 H1 in H.
+  case Hsplitl : (split_expr_non_passive ref_tgt t_tgt false) => [lhsl|]; rewrite Hsplitl in H; try discriminate.
+  case Hsplitr : (split_expr_non_passive ref_src t_src false) => [rhsl|]; rewrite Hsplitr in H; try discriminate.
+  case Hadd : (add_expr_connect_non_passive v_tgt v_src lhsl rhsl var2exprs0) => [newv2e|]; rewrite Hadd in H; try discriminate.
+  inversion H; clear H.
+  rewrite H4 in Hadd; clear H4.
+  intros n Hn.
+  case Hnthl : (nth_error lhsl n) => [[refl bl]|].
+  case Hb : bl.
+  case Hnthr : (nth_error rhsl n) => [[refr br]|].
+  assert (br = bl).
+  admit.
+  rewrite H Hb.
+
+  (*apply nth_error_Some in Hn.*)
+Admitted.
+
+Lemma base_ref_cepfind : forall ref n pv ft tmap checkt, base_ref ref tmap = Some (pv, ft) -> CEP.find (pv.1, 0%num) tmap = Some checkt -> 
+  ft_find_sub checkt (pv.2 + N.of_nat n) = ft_find_sub ft (N.of_nat n).
+Proof.
 Admitted.
 
 Lemma InferWidths_fun_correct : forall (hfs : HiFP.hfstmt) (inferorder : seq ProdVarOrder.t) (var2exprs : var2exprsmap) (tmap newtm : CEP.t ftype),
@@ -1451,35 +1989,27 @@ Proof.
   split. 
   admit. (* 对connection语句的要求 *)
 
-  assert (forall ft te, (forall n gt gte, n < tmap_type_size ft -> ft_find_sub ft (N.of_nat n) = Some gt -> ft_find_sub te (N.of_nat n) = Some gte ->
-        connect_fgtyp_compatible gt gte) ->
-    check_connect_fgtyp_compatible ft te (tmap_type_size ft)).
-  admit.
-
+  specialize check_connect_fgtyp_compatible4n as H.
   apply H; clear H.
-  intros n gt gte Hn Hlhs Hrhs.
-  assert ((tgt.1.1, N.add tgt.1.2 (N.of_nat n)) \in inferorder).
+  admit. (* tgt为false不允许flip是正确连接的要求 *)
+  intros n gt gte Hn Hflip Hlhs Hrhs.
+  assert (exists order1 order2, (inferorder = order1 ++ ((tgt.1.1, N.add tgt.1.2 (N.of_nat n)) :: order2)) 
+    /\ ((tgt.1.1, N.add tgt.1.2 (N.of_nat n)) \notin order1) 
+    /\ ((tgt.1.1, N.add tgt.1.2 (N.of_nat n)) \notin order2)).
   admit. (* inferorder 的正确性，是展开时的标号 *)
-  assert (exists order1 order2, inferorder = order1 ++ ((tgt.1.1, N.add tgt.1.2 (N.of_nat n)) :: order2) /\ ~ (tgt.1.1, N.add tgt.1.2 (N.of_nat n)) \in order1 /\ ~ (tgt.1.1, N.add tgt.1.2 (N.of_nat n)) \in order2).
-  admit. (* 由H推出 *)
-  clear H.
-  move : H0 => [order1 [order2 [H [Horder1 Horder2]]]].
-  rewrite H in Hinfer; rewrite /InferWidths_fun in Hinfer.
+  move : H => [order1 [order2 [H [Horder1 Horder2]]]].
+  rewrite H in Hinfer.
   case Hinfer1 : (InferWidths_fun order1 var2exprs tmap) => [tmap'|].
+
   assert (Hinfer2 : InferWidths_fun ((tgt.1.1, N.add tgt.1.2 (N.of_nat n)) :: order2) var2exprs tmap' = Some newtm).
-  admit. (* 由 Hinfer Hinfer1 *)
+  move : Hinfer Hinfer1.
+  apply infer_cons_order.
   clear Hinfer.
   simpl in Hinfer2.
   case Hel : (module_graph_vertex_set_p.find (tgt.1.1, N.add tgt.1.2 (N.of_nat n)) var2exprs) => [el|]; rewrite Hel in Hinfer2; try done.
   case Hinfer : (InferWidth_fun (tgt.1.1, N.add tgt.1.2 (N.of_nat n)) el tmap') => [newtm'|]; rewrite Hinfer in Hinfer2; try discriminate.
 
-  assert (forall expr rhs_expr_ls t_expr newtm, type_of_hfexpr expr newtm = Some t_expr -> split_expr_connect expr t_expr = Some rhs_expr_ls ->  (* 这里可以加bool list用来判断flip *)
-            forall n, n < length rhs_expr_ls -> match List.nth_error rhs_expr_ls n, ft_find_sub t_expr (N.of_nat n) with
-                                    | Some texpr, Some gt => type_of_hfexpr texpr newtm = Some (Gtyp gt)
-                                    | _, _ => true
-                                    end). 
-  admit. (* split和typeofexpr的性质 *)
-
+  specialize split_expr_type_correct; intro.
   case Hsplit : (split_expr_connect expr t_expr) => [rhs_expr_ls|].
   apply H0 with (expr := expr) (rhs_expr_ls := rhs_expr_ls) (t_expr := t_expr) (newtm := newtm) (n := n) in Hsplit; try done; clear H0.
   case Htexpr : (nth_error rhs_expr_ls n) => [texpr|]; rewrite Htexpr in Hsplit.
@@ -1494,10 +2024,7 @@ Proof.
   rewrite Hsub0 in Horder2; clear Hsub0.
   simpl in Horder2.
 
-  assert (forall ref n pv ft tmap, base_ref ref tmap = Some (pv, ft) -> CEP.find (tgt.1.1, 0%num) tmap = Some checkt -> ft_find_sub checkt (tgt.1.2 + N.of_nat n) = ft_find_sub tgt.2 (N.of_nat n)).
-  admit. (* 两种返回ftype函数的关系和正确性 *)
-
-  specialize H0 with (ref := ref) (n := n) (pv := tgt.1) (ft := tgt.2) (tmap := newtm).
+  specialize base_ref_cepfind with (ref := ref) (n := n) (pv := tgt.1) (ft := tgt.2) (tmap := newtm); intro.
   apply H0 in Htgt; clear H0; try done.
   rewrite Htgt in Horder2; clear Htgt.
   rewrite Hlhs in Horder2; clear Hlhs.
@@ -1519,17 +2046,15 @@ Proof.
   move /andP : Hinfer => [Hinfer _]; done.
 
   admit. (* type_of_hfexpr 不为None，由Htgt0 *)
-  admit. (* eta_expand这是啥，有Hbase *)
+  rewrite -surjective_pairing; done.
   admit. (* 由Htgt0不为None *)
   admit. (* 由 n < tmap_type_size tgt.2 知Hsub0不为None *)
   admit. (* 被连接的应该已被声明，find不为None *)
   admit. (* var2exprs应当满足的性质，由add_expr_connect *)
-  admit. (* n 不超过 rhs_expe_ls 的长度，不为None *)
-  assert (length rhs_expr_ls = tmap_type_size tgt.2).
-  admit. (* 由split_expr_connect的性质 *)
-  rewrite H0; clear H0; done.
+  admit. (* n 不超过 rhs_expr_ls 的长度，不为None *)
   admit. (* expr应该与t_expr匹配，不会出错 *)
   admit. (* 若infer order1有错误，则infer没有结果 *)
+  admit. (* 正确连接的前提 *)
 
   (* 所有passive的expr都一样 *)
   admit.
@@ -1547,36 +2072,9 @@ Proof.
   split. 
   admit. (* 对connection语句的要求 *)
 
-  assert (forall ft te, (forall n gt gte, n < tmap_type_size ft -> ft_find_sub ft (N.of_nat n) = Some gt -> ft_find_sub te (N.of_nat n) = Some gte ->
-        match ft_check_flip ft (N.of_nat n) false with
-        | Some false => connect_fgtyp_compatible gt gte
-        | Some true => connect_fgtyp_compatible gte gt
-        | None => false
-        end) ->
-        check_connect_non_passive_fgtyp ft te (tmap_type_size ft)).
-  admit.
-
-  apply H; clear H.
+  apply check_connect_non_passive_fgtyp4n.
   intros n gt gte Hn Hlhs Hrhs.
-
-  (* stop here, 在拆开infer之前，应该确定lhs or rhs的pv in inferorder *)
-  (* TBD!! *)
-  
-  assert ((v_tgt.1, N.add v_tgt.2 (N.of_nat n)) \in inferorder).
-  admit. (* inferorder 的正确性，是展开时的标号 *)
-  assert (exists order1 order2, inferorder = order1 ++ ((v_tgt.1, N.add v_tgt.2 (N.of_nat n)) :: order2) /\ ~ (v_tgt.1, N.add v_tgt.2 (N.of_nat n)) \in order1 /\ ~ (v_tgt.1, N.add v_tgt.2 (N.of_nat n)) \in order2).
-  admit. (* 由H推出 *)
-  clear H.
-  move : H0 => [order1 [order2 [H [Horder1 Horder2]]]].
-  rewrite H in Hinfer; rewrite /InferWidths_fun in Hinfer.
-  case Hinfer1 : (InferWidths_fun order1 var2exprs tmap) => [tmap'|].
-  assert (Hinfer2 : InferWidths_fun ((v_tgt.1, N.add v_tgt.2 (N.of_nat n)) :: order2) var2exprs tmap' = Some newtm).
-  admit. (* 由 Hinfer Hinfer1 *)
-  clear Hinfer.
-  simpl in Hinfer2.
-  case Hel : (module_graph_vertex_set_p.find (v_tgt.1, N.add v_tgt.2 (N.of_nat n)) var2exprs) => [el|]; rewrite Hel in Hinfer2; try done.
-  case Hinfer : (InferWidth_fun (v_tgt.1, N.add v_tgt.2 (N.of_nat n)) el tmap') => [newtm'|]; rewrite Hinfer in Hinfer2; try discriminate.
-
+  (* TBD!! stop here *)
   assert (forall ref_tgt ref_src t_tgt t_src v_tgt v_src tmap, base_ref ref_tgt tmap = Some (v_tgt, t_tgt) -> base_ref ref_src tmap = Some (v_src, t_src) ->
               match split_expr_non_passive ref_tgt t_tgt false, split_expr_non_passive ref_src t_src false with
               | Some lhsl, Some rhsl => (forall n, n < length lhsl -> match List.nth_error lhsl n, List.nth_error rhsl n with
@@ -1593,13 +2091,16 @@ Proof.
               | _, _ => false
               end). 
   admit. (* split和存var2exprs的性质 *)
-  apply H0 with (ref_tgt := ref) (t_tgt := t_tgt) (v_tgt := v_tgt) (ref_src := ref0) (t_src := t_src) (v_src := v_src) in Htgt; try done; clear H0.
+  (*specialize split_non_passive_correct as H.*)
+  generalize Htgt.
+  apply H with (ref_tgt := ref) (t_tgt := t_tgt) (v_tgt := v_tgt) (ref_src := ref0) (t_src := t_src) (v_src := v_src) in Htgt; try done; clear H.
   case Hsplit_lhs : (split_expr_non_passive ref t_tgt false) => [lhsl|]; rewrite Hsplit_lhs in Htgt.
   case Hsplit_rhs : (split_expr_non_passive ref0 t_src false) => [rhsl|]; rewrite Hsplit_rhs in Htgt.
   assert (length lhsl = tmap_type_size t_tgt).
   admit.
-  rewrite H0 in Htgt; clear H0.
+  rewrite H in Htgt; clear H.
   apply Htgt in Hn; clear Htgt.
+  move => Htgt.
   
   case Hlhsl : (nth_error lhsl n) => [[ref1 b1]|]; rewrite Hlhsl in Hn.
   case Hrhsl : (nth_error rhsl n) => [[ref2 b2]|]; rewrite Hrhsl in Hn.
@@ -1609,20 +2110,95 @@ Proof.
   assert (b1 = b2). (* tgt和src类型相同 *)
   admit.
 
-  case Hb : b1; rewrite Hb in H0 Hn H1; rewrite -H0; rewrite -H1 in Hn.
+  case Hb : b1; rewrite Hb in H0 Hn H; rewrite -H; rewrite -H0 in Hn.
   (* case1 : flip field *)
+  assert ((v_src.1, N.add v_src.2 (N.of_nat n)) \in inferorder).
+  admit. (* inferorder 的正确性，是展开时的标号 *)
+  assert (exists order1 order2, inferorder = order1 ++ ((v_src.1, N.add v_src.2 (N.of_nat n)) :: order2) /\ ~ (v_src.1, N.add v_src.2 (N.of_nat n)) \in order1 /\ ~ (v_src.1, N.add v_src.2 (N.of_nat n)) \in order2).
+  admit. (* 由H1推出 *)
+  clear H1.
+  move : H2 => [order1 [order2 [H2 [Horder1 Horder2]]]].
+  rewrite H2 in Hinfer; rewrite /InferWidths_fun in Hinfer.
+  case Hinfer1 : (InferWidths_fun order1 var2exprs tmap) => [tmap'|].
+  assert (Hinfer2 : InferWidths_fun ((v_src.1, N.add v_src.2 (N.of_nat n)) :: order2) var2exprs tmap' = Some newtm).
+  admit. (* 由 Hinfer Hinfer1 *)
+  clear Hinfer.
+  simpl in Hinfer2.
+  case Hel : (module_graph_vertex_set_p.find (v_src.1, N.add v_src.2 (N.of_nat n)) var2exprs) => [el|]; rewrite Hel in Hinfer2; try done.
+  case Hinfer : (InferWidth_fun (v_src.1, N.add v_src.2 (N.of_nat n)) el tmap') => [newtm'|]; rewrite Hinfer in Hinfer2; try discriminate.
+
   apply InferWidth_fun_correct with (pv := (v_src.1, (v_src.2 + N.of_nat n)%num)) (el := el) (tmap := tmap') (newtm := newtm') (expr := (Eref ref1)) in Hinfer.
   simpl in Hinfer.
-  case Htgt0 : (CEP.find (tgt.1.1, 0%num) newtm') => [checkt'|]; rewrite Htgt0 in Hinfer.
-  case Hsub0 : (ft_find_sub checkt' (tgt.1.2 + N.of_nat n)) => [nt|]; rewrite Hsub0 in Hinfer.
-  case Htgt : (CEP.find (tgt.1.1, 0%num) newtm) => [checkt|].
-  apply inferwidths_ls with (var2exprs := var2exprs) (tmap := newtm') (tmap' := newtm) (checkt := checkt') (checkt' := checkt) in Horder2; try done.
-  rewrite Hsub0 in Horder2; clear Hsub0.
-  simpl in Horder2.
+  case Hsrc0 : (CEP.find (v_src.1, 0%num) newtm') => [checkt'|]; rewrite Hsrc0 in Hinfer.
+  case Hsub0 : (ft_find_sub checkt' (v_src.2 + N.of_nat n)) => [nt|]; rewrite Hsub0 in Hinfer.
+  case Htgt0 : (base_ref ref1 newtm') => [[v_tgt0 t_tgt0]|]; rewrite Htgt0 in Hinfer.
 
-  assert (forall ref n pv ft tmap, base_ref ref tmap = Some (pv, ft) -> CEP.find (tgt.1.1, 0%num) tmap = Some checkt -> ft_find_sub checkt (tgt.1.2 + N.of_nat n) = ft_find_sub tgt.2 (N.of_nat n)).
-  admit. (* 两种返回ftype函数的关系和正确性 *)
+  (* 下面证t_tgt0 = gt和gte = Gtyp nt *)
+  assert ((Gtyp gt) = t_tgt0).
+  move : Htgt Hsplit_lhs Hlhs Hlhsl Htgt0.
+  admit. (* split之后取算n个expr的类型 = 整个expr类型的第n个field *) (* base_ref ref1 newtm' = base_ref ref1 newtm, 由于v_tgt0不在order2中 *)
+  assert (gte = nt).
+  move : Hsrc Hsrc0 Hsub0 Hrhs.
+  admit.
+  rewrite -H1 -H3 in Hinfer; rewrite /connect_type_compatible in Hinfer.
+  assert (fgtyp_equiv gte gt).
+  admit. (* 由t_tgt t_src 应该ftype_equiv得到 *) 
+  apply Hinfer in H4; clear Hinfer.
+  move /andP : H4 => [_ H4].
+  simpl in H4.
+  move /andP : H4 => [H4 _]; done.
 
+  admit.
+  admit.
+  admit.
+  admit. (* var2exprs正确性的结论 *)
+  admit.
+
+  (* case2 : Nflip *)
+  assert ((v_tgt.1, N.add v_tgt.2 (N.of_nat n)) \in inferorder).
+  admit. (* inferorder 的正确性，是展开时的标号 *)
+  assert (exists order1 order2, inferorder = order1 ++ ((v_tgt.1, N.add v_tgt.2 (N.of_nat n)) :: order2) /\ ~ (v_tgt.1, N.add v_tgt.2 (N.of_nat n)) \in order1 /\ ~ (v_tgt.1, N.add v_tgt.2 (N.of_nat n)) \in order2).
+  admit. (* 由H推出 *)
+  clear H1.
+  move : H2 => [order1 [order2 [H2 [Horder1 Horder2]]]].
+  rewrite H2 in Hinfer; rewrite /InferWidths_fun in Hinfer.
+  case Hinfer1 : (InferWidths_fun order1 var2exprs tmap) => [tmap'|].
+  assert (Hinfer2 : InferWidths_fun ((v_tgt.1, N.add v_tgt.2 (N.of_nat n)) :: order2) var2exprs tmap' = Some newtm).
+  admit. (* 由 Hinfer Hinfer1 *)
+  clear Hinfer.
+  simpl in Hinfer2.
+  case Hel : (module_graph_vertex_set_p.find (v_tgt.1, N.add v_tgt.2 (N.of_nat n)) var2exprs) => [el|]; rewrite Hel in Hinfer2; try done.
+  case Hinfer : (InferWidth_fun (v_tgt.1, N.add v_tgt.2 (N.of_nat n)) el tmap') => [newtm'|]; rewrite Hinfer in Hinfer2; try discriminate.
+
+  apply InferWidth_fun_correct with (pv := (v_tgt.1, N.add v_tgt.2 (N.of_nat n))) (el := el) (tmap := tmap') (newtm := newtm') (expr := (Eref ref2)) in Hinfer.
+  simpl in Hinfer.
+  case Htgt0 : (CEP.find (v_tgt.1, 0%num) newtm') => [checkt'|]; rewrite Htgt0 in Hinfer.
+  case Hsub0 : (ft_find_sub checkt' (v_tgt.2 + N.of_nat n)) => [nt|]; rewrite Hsub0 in Hinfer.
+  case Hsrc0 : (base_ref ref2 newtm') => [[v_src0 t_src0]|]; rewrite Hsrc0 in Hinfer.
+
+  (* 下面证t_tgt0 = gt和gte = Gtyp nt *)
+  assert ((Gtyp gte) = t_src0).
+  admit. 
+  assert (gt = nt).
+  admit.
+  rewrite -H1 -H3 in Hinfer; rewrite /connect_type_compatible in Hinfer.
+  assert (fgtyp_equiv gt gte).
+  admit. (* 由t_tgt t_src 应该ftype_equiv得到 *) 
+  apply Hinfer in H4; clear Hinfer.
+  move /andP : H4 => [_ H4].
+  simpl in H4.
+  move /andP : H4 => [H4 _]; done.
+
+  admit.
+  admit.
+  admit.
+  admit. (* var2exprs正确性的结论 *)
+  admit.
+  admit.
+  admit.
+  admit.
+  admit.
+  admit.
 Admitted.
 
 Definition InferWidths_m F :=
@@ -1645,7 +2221,7 @@ Fixpoint fillft_vm (n : nat) (ft : ftype) (pv : ProdVarOrder.t) (vmap : module_g
    | 0 => Some ft
    | S m => match module_graph_vertex_set_p.find (fst pv, (N.add (snd pv) (N.of_nat m))) vmap with
             | Some nt => match List.hd_error (input_connectors nt) with
-                        | Some gt => match ft_set_sub (fst pv, (N.add (snd pv) (N.of_nat m))) ft (Gtyp gt) (snd pv) with
+                        | Some gt => match ft_set_sub ft gt (N.of_nat m) with
                                    | Some nft => fillft_vm m nft pv vmap
                                    | None => None
                                    end
@@ -1805,18 +2381,1105 @@ Fixpoint type_of_hfexpr_vm (vmap : module_graph_vertex_set_p.env) (e : HiFP.hfex
    | _ => None (* Some (Gtyp (Fuint 0)) *)
    end.
 
-Lemma InferWidths_fun_correct' F : forall vmap inferorder var2exprs tmap ct, Sem F vmap ct -> 
-  forall v, v \in inferorder -> 
-        match module_graph_vertex_set_p.find v vmap, module_graph_vertex_set_p.find v var2exprs, CEP.find (fst v, N0) tmap with
-        | Some nt, Some el, Some init => match List.hd_error (input_connectors nt), fil_ftlist (map (fun e => type_of_hfexpr_vm vmap e tmap) el), ft_find_sub v init N0 with
-                    | Some gt, Some eftl, Some (Gtyp initt) => match max_ftlist eftl initt with
-                                                        | Some nt => sizeof_fgtyp gt >= sizeof_fgtyp nt
-                                                        | _ => true
+Fixpoint unfold_Swhen (s : HiFP.hfstmt) : HiFP.hfstmt_seq :=
+  match s with
+  | Swhen _ ss_t ss_f => Qcat (unfold_Swhens ss_t) (unfold_Swhens ss_f)
+  | _ => Qcons s (Qnil HiFirrtl.ProdVarOrder.T)
+  end
+  with unfold_Swhens (ss : HiFP.hfstmt_seq) : HiFP.hfstmt_seq :=
+  match ss with
+  | Qnil => (Qnil HiFirrtl.ProdVarOrder.T)
+  | Qcons s ss' => Qcat (unfold_Swhen s) (unfold_Swhens ss')
+  end.
+
+Definition Sem_port' (p : HiFP.hfport) (vm : module_graph_vertex_set_p.env) : Prop :=
+(* The predicate returns true if the vertex set V conforms to the sequence of ports pp. *)
+  match p with
+  | Foutput v t => (forall n : nat, if n < (tmap_type_size t) then
+                    match ft_find_sub t (N.of_nat n) with
+                    | Some nv => module_graph_vertex_set_p.find (fst v, N.of_nat n) vm = Some (InPort nv)
+                    | None => false
+                    end else true)
+  | _ => true
+   end.
+
+Fixpoint Sem_frag_stmt' (vm : module_graph_vertex_set_p.env) (s : HiFP.hfstmt) (tmap : CEP.t ftype) : Prop :=
+   (* The predicate returns True if vm_new/ct_new can be constructed from vm_old/ct_old by applying s. 
+   type checking, constraints *)
+  match s with
+  | Sfcnct ref_tgt (Eref ref_src) => (* allow non-passive types *)
+            match type_of_hfexpr_vm vm (Eref ref_tgt) tmap, type_of_hfexpr_vm vm (Eref ref_src) tmap with
+            | Some t_tgt, Some t_src => connect_non_passive_type t_tgt t_src
+            | _, _ => False
+            end
+  | Sfcnct ref expr => 
+            match type_of_hfexpr_vm vm (Eref ref) tmap, type_of_hfexpr_vm vm expr tmap with
+            | Some t_tgt, Some t_src => connect_type_compatible t_tgt t_src
+            | _, _ => False
+            end
+  | Sreg v reg => (if (reset reg) is (Rst rst_sig rst_val)
+                  then match type_of_hfexpr_vm vm rst_val tmap with
+                  | Some t_src => connect_type_compatible (type reg) t_src
+                  | _ => False
+                  end
+                  else True) /\
+                  (forall n : nat, n < (tmap_type_size (type reg)) ->
+                          match ft_find_sub (type reg) (N.of_nat n) with
+                          | Some nv => match reset reg with
+                                      | NRst => module_graph_vertex_set_p.find (fst v, N.of_nat n) vm = Some (Register nv)
+                                      | Rst rst_sig _ => match type_of_hfexpr_vm vm rst_sig tmap with
+                                                        | Some (Gtyp Fasyncreset) => module_graph_vertex_set_p.find (fst v, N.of_nat n) vm = Some (RegisterReset nv true)
+                                                        | Some (Gtyp (Fuint 1)) => module_graph_vertex_set_p.find (fst v, N.of_nat n) vm = Some (RegisterReset nv false)
+                                                        | _ => False
                                                         end
-                    | _,_,_ => true
+                                      end
+                          | None => False
+                          end)
+  | Swire v t => (forall n : nat, if n < (tmap_type_size t) then
+                          match ft_find_sub t (N.of_nat n) with
+                          | Some nv => module_graph_vertex_set_p.find (fst v, N.of_nat n) vm = Some (Wire nv)
+                          | None => False
+                          end else True)
+  | Snode v e => match type_of_hfexpr_vm vm e tmap with
+                | Some te => (forall n : nat, if n < (tmap_type_size te) then
+                          match ft_find_sub te (N.of_nat n) with
+                          | Some nv => module_graph_vertex_set_p.find (fst v, N.of_nat n) vm = Some (Node nv)
+                          | None => False
+                          end else True)
+                | None => False
+                end
+  | Swhen _ s1 s2 => Sem_frag_stmts' vm s1 tmap /\ Sem_frag_stmts' vm s2 tmap
+  | _ => True 
+  end
+with Sem_frag_stmts' (vm : module_graph_vertex_set_p.env) (ss : HiFP.hfstmt_seq) (tmap : CEP.t ftype) : Prop :=
+  match ss with
+  | Qnil => True
+  | Qcons s ss' => Sem_frag_stmt' vm s tmap /\ Sem_frag_stmts' vm ss' tmap
+  end.
+
+Lemma geq_conj2mux : forall vmap tmap (gt initt : fgtyp) (el : seq HiFP.hfexpr) eftl (nt : fgtyp), (forall (texpr : HiFP.hfexpr) (tge : fgtyp), texpr \in el -> type_of_hfexpr_vm vmap texpr tmap = Some (Gtyp tge) -> ((sizeof_fgtyp gt) >= (sizeof_fgtyp tge))) ->
+        fil_ftlist [seq type_of_hfexpr_vm vmap e tmap | e <- el] = Some eftl -> sizeof_fgtyp initt = 0 -> max_ftlist eftl initt = Some nt -> ((sizeof_fgtyp gt) >= (sizeof_fgtyp nt)).
+Proof.
+  intros vmap tmap gt initt.
+  elim.
+  intros.
+  simpl in H0.
+  inversion H0; clear H0.
+  rewrite -H4 in H2.
+  simpl in H2.
+  inversion H2; clear H2.
+  rewrite -H3 H1.
+  rewrite /sizeof_fgtyp.
+  case Het : gt; try done.
+
+  intros hd tl IH eftl nt H Heftl Hinitt Hmax.
+  simpl in Heftl.
+  case Hhd : (type_of_hfexpr_vm vmap hd tmap) => [f|]; rewrite Hhd in Heftl; try discriminate.
+  case Hf : f => [hdt||]; rewrite Hf in Hhd Heftl; clear Hf; try discriminate.
+  case Heftl' : (fil_ftlist [seq type_of_hfexpr_vm vmap e tmap | e <- tl]) => [eftl'|]; rewrite Heftl' in Heftl; try discriminate.
+  inversion Heftl; clear Heftl.
+  rewrite -H1 in Hmax.
+  simpl in Hmax.
+  case Hmax' : (max_ftlist eftl' initt) => [nt'|]; rewrite Hmax' in Hmax; try discriminate.
+
+  assert (max_fgtyp hdt nt' = Some nt -> sizeof_fgtyp nt' <= sizeof_fgtyp gt -> sizeof_fgtyp hdt <= sizeof_fgtyp gt -> sizeof_fgtyp nt <= sizeof_fgtyp gt).
+  clear.
+  intros.
+  rewrite /max_fgtyp in H.
+  case Hhd : hdt => [w|w|w|w|||]; rewrite Hhd in H H1; try discriminate.
+  case Hnt' : nt' => [w'|w'|w'|w'|||]; rewrite Hnt' in H H0; try discriminate.
+  inversion H; clear H.
+  simpl in H1; simpl in H0; simpl.
+  move : H1 H0.
+  admit.
+  case Hnt' : nt' => [w'|w'|w'|w'|||]; rewrite Hnt' in H H0; try discriminate.
+  inversion H; clear H.
+  simpl in H1; simpl in H0; simpl.
+  move : H1 H0.
+  admit.
+  case Hnt' : nt' => [w'|w'|w'|w'|||]; rewrite Hnt' in H H0; try discriminate.
+  inversion H; clear H.
+  simpl in H1; simpl in H0; simpl.
+  move : H1 H0.
+  admit.
+  case Hnt' : nt' => [w'|w'|w'|w'|||]; rewrite Hnt' in H H0; try discriminate.
+  inversion H; clear H.
+  simpl in H1; simpl in H0; simpl.
+  move : H1 H0.
+  admit.
+
+  apply H0 in Hmax; try done; clear H0.
+  apply IH with (eftl := eftl'); try done.
+  intros expr tge Hin.
+  apply H.
+  rewrite in_cons Hin.
+  rewrite orb_true_r; done.
+  apply H with (texpr := hd); try done.
+  rewrite in_cons.
+  rewrite eq_refl.
+  rewrite orb_true_l; done.
+Admitted.
+
+Lemma split_expr_type_vm_correct : forall expr rhs_expr_ls t_expr newtm vm, 
+  type_of_hfexpr_vm vm expr newtm = Some t_expr -> split_expr_connect expr t_expr = Some rhs_expr_ls ->
+  forall n, match ft_find_sub t_expr (N.of_nat n), List.nth_error rhs_expr_ls n with
+            | Some gt, Some texpr => type_of_hfexpr_vm vm texpr newtm = Some (Gtyp gt)
+            | _, _ => true
+            end.
+Proof.
+Admitted.
+
+Fixpoint find_sub_expr (pv : ProdVarOrder.t) (s : HiFP.hfstmt) (tmap : CEP.t ftype) : option (seq HiFP.hfexpr) :=
+  match s with
+  | Sreg v r => if (pv.1 == v.1) then match reset r with
+                | NRst => Some nil
+                | Rst _ rst_val => match split_expr_connect rst_val (type r) with
+                                  | Some rstl => match List.nth_error rstl (N.to_nat pv.2) with
+                                                | Some e => Some [::e]
+                                                | None => None
+                                                end
+                                  | None => None
+                                  end
+                end
+                else Some nil
+  | Snode v e => if (pv.1 == v.1) then match type_of_hfexpr e tmap with
+                | Some t => match split_expr_connect e t with
+                            | Some rstl => match List.nth_error rstl (N.to_nat pv.2) with
+                                                | Some e => Some [::e]
+                                                | None => None
+                                                end
+                            | None => None
+                            end
+                | _ => None
+                end
+                else Some nil
+  | Sfcnct ref_tgt (Eref ref_src) =>
+                match base_ref ref_tgt tmap, base_ref ref_src tmap with
+                | Some (v_tgt, t_tgt), Some (v_src, t_src) =>
+                  if (pv.1 == v_tgt.1) then match split_expr_non_passive ref_src t_src false with
+                                          | Some rhsl => match List.nth_error rhsl ((N.to_nat pv.2) - (N.to_nat v_tgt.2)) with
+                                                        | Some (refr, false) => Some [::(Eref refr)]
+                                                        | Some (_, true) => Some nil
+                                                        | _ => None
+                                                        end
+                                          | _ => None
+                                          end
+                  else if (pv.1 == v_src.1) then match split_expr_non_passive ref_tgt t_tgt false with
+                                          | Some lhsl => match List.nth_error lhsl ((N.to_nat pv.2) - (N.to_nat v_src.2)) with
+                                                        | Some (refl, true) => Some [::(Eref refl)]
+                                                        | Some (_, false) => Some nil
+                                                        | _ => None
+                                                        end
+                                          | _ => None
+                                          end
+                  else Some nil
+                | _, _ => None
+                end
+  | Sfcnct ref_tgt expr_src =>
+                match base_ref ref_tgt tmap, type_of_hfexpr expr_src tmap with
+                | Some (v, t_tgt), Some t_src =>
+                    if (pv.1 == v.1)
+                      then match split_expr_connect expr_src t_src with
+                      | Some rstl => match List.nth_error rstl ((N.to_nat pv.2) - (N.to_nat v.2)) with
+                                    | Some e => Some [::e]
+                                    | None => None
+                                    end
+                      | None => None
+                      end
+                    else Some nil
+                | _,_ => None
+                end
+  | Swhen _ s1 s2 => match find_sub_exprs pv s1 tmap, find_sub_exprs pv s2 tmap with
+                    | Some e1, Some e2 => Some (e1 ++ e2)
+                    | _,_ => None
                     end
-        | _,_,_ => true
-        end.
+  | _ => Some nil
+  end
+with find_sub_exprs (v : ProdVarOrder.t) (ss : HiFP.hfstmt_seq) (tmap : CEP.t ftype) : option (seq HiFP.hfexpr) :=
+  match ss with
+  | Qnil => Some nil
+  | Qcons s ss' => match find_sub_expr v s tmap, find_sub_exprs v ss' tmap with
+                  | Some e, Some el => Some (e ++ el)
+                  | _, _ => None
+                  end
+  end.
+
+Lemma ftype2fgtyp_compatible : forall ft te n, connect_type_compatible ft te -> 
+  match ft_check_flip ft n false, ft_find_sub ft n, ft_find_sub te n with
+  | Some false, Some gt, Some gte => connect_fgtyp_compatible gt gte
+  (*| Some true, Some gt, Some gte => connect_fgtyp_compatible gte gt*)
+  | _,_,_ => true
+  end.
 Proof.
   
-Qed.
+Admitted.
+
+Lemma ftype2fgtyp_non_passive_compatible : forall ft te n, connect_non_passive_type ft te -> 
+  match ft_check_flip ft n false, ft_find_sub ft n, ft_find_sub te n with
+  | Some false, Some gt, Some gte => connect_fgtyp_compatible gt gte
+  | Some true, Some gt, Some gte => connect_fgtyp_compatible gte gt
+  | _,_,_ => true
+  end.
+Proof.
+  
+Admitted.
+
+Lemma component_vx_type_vm : forall v r tmap vmap v_tgt t_tgt t_tgt' gte, base_ref r tmap = Some (v_tgt, t_tgt) -> if (v.1 == v_tgt.1) then fillft_vm (tmap_type_size t_tgt) t_tgt v_tgt vmap = Some t_tgt' -> ft_find_sub t_tgt' (N.sub v.2 v_tgt.2) = Some gte ->
+  match module_graph_vertex_set_p.find v vmap with
+  | Some (OutPort gt) 
+  | Some (Register gt) 
+  | Some (RegisterReset gt _) 
+  | Some (Wire gt) 
+  | Some (Node gt) => gt = gte
+  | _ => true
+  end
+  else true.
+Proof.
+Admitted.
+
+Lemma fillft_vm_nth_eq : forall r v t t' rstl refr b n vmap tmap gt, base_ref r tmap = Some (v, t) -> split_expr_non_passive r t false = Some rstl -> 
+  nth_error rstl n = Some (refr, b) -> fillft_vm (tmap_type_size t) t v vmap = Some t' -> type_of_hfexpr_vm vmap (Eref refr) tmap = Some (Gtyp gt) -> ft_find_sub t' (N.of_nat n) = Some gt.
+Proof.
+Admitted.
+
+Lemma type_of_hfexpr_vm_eq : forall e tmap vmap t_src tev, type_of_hfexpr e tmap = Some t_src -> type_of_hfexpr_vm vmap e tmap = Some tev -> ftype_equiv t_src tev.
+Proof.
+  
+Admitted.
+
+Lemma split_non_passive_flip_eq : forall r t n rstl p, split_expr_non_passive r t false = Some rstl -> nth_error rstl n = Some p -> Some p.2 = ft_check_flip t (N.of_nat n) false.
+Proof.
+Admitted.
+
+Lemma fillft_vm_eq : forall t t' v vmap, fillft_vm (tmap_type_size t) t v vmap = Some t' -> ftype_equiv t t'.
+Proof.
+Admitted.
+
+Lemma Sem_frag_stmt_correct4r : forall s vmap tmap, Sem_frag_stmt' vmap s tmap -> 
+  forall (v : ProdVarOrder.t), match find_sub_expr v s tmap with
+  | Some el => match module_graph_vertex_set_p.find v vmap with
+              | Some (OutPort gt) 
+              | Some (Register gt) 
+              | Some (RegisterReset gt _) 
+              | Some (Wire gt) 
+              | Some (Node gt) => forall e te, e \in el -> type_of_hfexpr_vm vmap e tmap = Some (Gtyp te) -> connect_fgtyp_compatible gt te
+              | _ => true
+              end
+  | _ => true
+  end
+with Sem_frag_stmts_correct4r : forall ss vmap tmap, Sem_frag_stmts' vmap ss tmap -> 
+  forall (v : ProdVarOrder.t), match find_sub_exprs v ss tmap with
+  | Some el => match module_graph_vertex_set_p.find v vmap with
+              | Some (OutPort gt) 
+              | Some (Register gt) 
+              | Some (RegisterReset gt _) 
+              | Some (Wire gt) 
+              | Some (Node gt) => forall e te, e \in el -> type_of_hfexpr_vm vmap e tmap = Some (Gtyp te) -> connect_fgtyp_compatible gt te
+              | _ => true
+              end
+  | _ => true
+  end.
+Proof.
+  clear Sem_frag_stmt_correct4r.
+  intros.
+  case Hs : s => [|r t|r reg|||r e|r e|r|c s1 s2]; rewrite Hs in H; simpl in H; simpl.
+  - (* skip *)
+    clear Sem_frag_stmts_correct4r.
+    case Hv : (module_graph_vertex_set_p.find v vmap) => [vx|]; try done.
+    case Hgt : vx => [gt|||||||||||||||||||||||||||||||||||||gt|gt|gt|gt|]; try done.
+  - (* wire *)
+    clear Sem_frag_stmts_correct4r.
+    case Hv : (module_graph_vertex_set_p.find v vmap) => [vx|]; try done.
+    case Hgt : vx => [gt|||||||||||||||||||||||||||||||||||||gt|gt|gt|gt|]; try done.
+  - (* reg *)
+    clear Sem_frag_stmts_correct4r.
+    case Hr : (v.1 == r.1); try done.
+    case Hrst : (reset reg) => [|rst_sig rst_val]; rewrite Hrst in H; try done.
+    (* Nrst *)
+    case Hv : (module_graph_vertex_set_p.find v vmap) => [vx|]; try done.
+    case Hgt : vx => [gt|||||||||||||||||||||||||||||||||||||gt|gt|gt|gt|]; try done.
+    (* Rst *)
+    move : H => [Hrst_val Hfind].
+    specialize Hfind with (n := N.to_nat v.2).
+    case Hsplit : (split_expr_connect rst_val (type reg)) => [rstl|]; try done.
+    case Hnth : (nth_error rstl (N.to_nat v.2)) => [e|]; try done.
+    case Hval : (type_of_hfexpr_vm vmap rst_val tmap) => [t_rst|]; rewrite Hval in Hrst_val;try done.
+    apply split_expr_type_vm_correct with (rhs_expr_ls := rstl) (n := (N.to_nat v.2)) in Hval; try done.
+    rewrite Nnat.N2Nat.id in Hval Hfind.
+    assert (N.to_nat v.2 < tmap_type_size (type reg)).
+    admit.
+    apply Hfind in H; clear Hfind.
+    case Hfindv : (ft_find_sub (type reg) v.2) => [gt|]; rewrite Hfindv in H; try done.
+    case H' : (type_of_hfexpr_vm vmap rst_sig tmap) => [a|]; rewrite H' in H; try done; clear H'.
+    case H' : (a) => [f0||]; rewrite H' in H; try done; clear H' a.
+    case H' : f0 => [n0||||||]; rewrite H' in H;try done; clear H' f0.
+    case H' : n0 => [|n1]; rewrite H' in H; try done; clear H' n0.
+    case H' : n1; rewrite H' in H; try done; clear H' n1.
+    move /eqP : Hr => Hr; rewrite -Hr in H.
+    rewrite -surjective_pairing in H.
+    rewrite H.
+    intros.
+    rewrite mem_seq1 in H0.
+    move /eqP : H0 => H0.
+    rewrite H0 in H1; clear H0.
+    apply ftype2fgtyp_compatible with (n := v.2) in Hrst_val.
+    assert (ft_check_flip (type reg) v.2 false = Some false).
+    admit. (* 除了fcnct，不考虑flip？重要！！ *)
+    rewrite H0 Hfindv in Hrst_val.
+    case Ht_rst : (ft_find_sub t_rst v.2) => [gte|]; rewrite Ht_rst in Hrst_val Hval.
+    rewrite Hnth H1 in Hval.
+    inversion Hval; done.
+    admit. (* must not be none *)
+      (* the same as sync reset *)
+      move /eqP : Hr => Hr; rewrite -Hr in H.
+      rewrite -surjective_pairing in H.
+      rewrite H.
+      intros.
+      rewrite mem_seq1 in H0.
+      move /eqP : H0 => H0.
+      rewrite H0 in H1; clear H0.
+      apply ftype2fgtyp_compatible with (n := v.2) in Hrst_val.
+      assert (ft_check_flip (type reg) v.2 false = Some false).
+      admit. (* 除了fcnct，不考虑flip？重要！！ *)
+      rewrite H0 Hfindv in Hrst_val.
+      case Ht_rst : (ft_find_sub t_rst v.2) => [gte|]; rewrite Ht_rst in Hrst_val Hval.
+      rewrite Hnth H1 in Hval.
+      inversion Hval; done.
+      admit. (* must not be none *)
+    rewrite /connect_type_compatible in Hrst_val.
+    move /andP : Hrst_val => [H _]. 
+    apply ftype_equiv_split_eq with (s := rst_val) in H.
+    rewrite -H Hsplit; done.
+    case Hv : (module_graph_vertex_set_p.find v vmap) => [vx|]; try done.
+    case Hgt : vx => [gt|||||||||||||||||||||||||||||||||||||gt|gt|gt|gt|]; try done.
+  - (* mem *)
+    admit.
+  - (* inst *)
+    admit.
+  - (* node *)
+    clear Sem_frag_stmts_correct4r.
+    case Hr : (v.1 == r.1); try done.
+    case Hte : (type_of_hfexpr e tmap) => [te|]; try done.
+    case Htev : (type_of_hfexpr_vm vmap e tmap) => [tev|]; rewrite Htev in H; try done. 
+    case Hsplit : (split_expr_connect e te) => [rstl|]; try done.
+    case Hnth : (nth_error rstl (N.to_nat v.2)) => [e0|]; try done.
+    specialize H with (n := N.to_nat v.2).
+    rewrite Nnat.N2Nat.id in H.
+    assert (N.to_nat v.2 < tmap_type_size tev).
+    admit.
+    rewrite H0 in H; clear H0.
+    case Hfindv : (ft_find_sub tev v.2) => [gt|]; rewrite Hfindv in H; try done.
+    move /eqP : Hr => Hr; rewrite -Hr in H.
+    rewrite -surjective_pairing in H.
+    rewrite H.
+    intros.
+    rewrite mem_seq1 in H0.
+    move /eqP : H0 => H0.
+    rewrite H0 in H1; clear H0.
+    apply split_expr_type_vm_correct with (rhs_expr_ls := rstl) (n := N.to_nat v.2) in Htev; try done.
+    rewrite Nnat.N2Nat.id in Htev.
+    rewrite Hfindv Hnth in Htev.
+    rewrite Htev in H1.
+    inversion H1; clear H1.
+    admit.
+    assert (ftype_equiv te tev).
+    admit.
+    apply ftype_equiv_split_eq with (s := e) in H0; rewrite -H0; done.
+    (* v.1 <> r.1 *)
+    case Hv : (module_graph_vertex_set_p.find v vmap) => [vx|]; try done.
+    case Hgt : vx => [gt|||||||||||||||||||||||||||||||||||||gt|gt|gt|gt|]; try done.
+  - (* fcnct *)
+    clear Sem_frag_stmts_correct4r.
+    case He : e => [t c| c e1 | u e1 | op e1 e2 | c e1 e2 | c e1 | r2 ]; rewrite He in H; try done.
+    - (* 普通connection *)
+      rewrite -He; rewrite -He in H.
+      case Hbase : (base_ref r tmap) => [[v_tgt t_tgt]|]; rewrite Hbase in H; try done.
+      case Hte : (type_of_hfexpr e tmap) => [t_src|]; try done.
+      case Hr : (v.1 == v_tgt.1); try done.
+      case Hsplit : (split_expr_connect e t_src) => [rstl|]; try done.
+      case Hnth : (nth_error rstl (N.to_nat v.2 - N.to_nat v_tgt.2)) => [e0|]; try done.
+      case Hfill : (fillft_vm (tmap_type_size t_tgt) t_tgt v_tgt vmap) => [t_tgt'|]; rewrite Hfill in H; try done.
+      case Hv : (module_graph_vertex_set_p.find v vmap) => [vx|]; try done.
+      case Hgt : vx => [gt|||||||||||||||||||||||||||||||||||||gt|gt|gt|gt|]; try done.
+      case Hgte : (ft_find_sub t_tgt' (N.sub v.2 v_tgt.2)) => [gte|].
+      apply component_vx_type_vm with (v := v) (vmap := vmap) (t_tgt' := t_tgt') (gte := gte) in Hbase; try done.
+      rewrite Hr in Hbase.
+      apply Hbase in Hfill; clear Hbase.
+      rewrite Hv Hgt in Hfill.
+      case Htev : (type_of_hfexpr_vm vmap e tmap) => [tev|]; rewrite Htev in H; try done.
+      intros.
+      rewrite mem_seq1 in H0.
+      move /eqP : H0 => H0.
+      rewrite H0 in H1; clear H0.
+      generalize Htev.
+      apply split_expr_type_vm_correct with (rhs_expr_ls := rstl) (n := N.to_nat v.2 - N.to_nat v_tgt.2) in Htev; try done.
+      rewrite <-Nnat.N2Nat.inj_sub in Htev; try done.
+      rewrite Nnat.N2Nat.id in Htev; try done.
+      move => Htev'.
+      rewrite -Hfill in Hgte; clear Hfill gte.
+      case Htnev : (ft_find_sub tev (v.2 - v_tgt.2)) => [gnt|]; rewrite Htnev in Htev.
+      rewrite <-Nnat.N2Nat.inj_sub in Hnth.
+      rewrite Hnth in Htev.
+      rewrite H1 in Htev; clear H1.
+      inversion Htev; clear Htev.
+      apply ftype2fgtyp_compatible with (n := (N.sub v.2 v_tgt.2)) in H; try done.
+      assert (ft_check_flip t_tgt' (v.2 - v_tgt.2) false = Some false).
+      admit.
+      rewrite H0 Hgte Htnev in H; done.
+      admit. (* 不是None *)
+      apply type_of_hfexpr_vm_eq with (vmap := vmap) (tev := tev) in Hte; try done.
+      apply ftype_equiv_split_eq with (s := e) in Hte.
+      rewrite Hte in Hsplit; done.
+      done.
+      admit. (* None *)
+
+      (* 相同的vx case *)
+      admit.
+      admit. 
+      admit. 
+      admit.
+      admit.
+      
+    - (* 同样的e case *)
+      admit.
+      admit.
+      admit.
+      admit.
+      admit.
+    - (* Eref *)
+      case Hbase : (base_ref r tmap) => [[v_tgt t_tgt]|]; rewrite Hbase in H; try done.
+      case Hbase2 : (base_ref r2 tmap) => [[v_src t_src]|]; rewrite Hbase2 in H; try done.
+      case Hr : (v.1 == v_tgt.1); try done.
+        (* lhs *)
+        case Hsplit : (split_expr_non_passive r2 t_src false) => [rstl|]; try done.
+        case Hnth : (nth_error rstl (N.to_nat v.2 - N.to_nat v_tgt.2)) => [[refr b]|]; try done.
+        case Hb : b; try done.
+        case Hv : (module_graph_vertex_set_p.find v vmap) => [vx|]; try done.
+        case Hgt : vx => [gt|||||||||||||||||||||||||||||||||||||gt|gt|gt|gt|]; try done.
+        case Hv : (module_graph_vertex_set_p.find v vmap) => [vx|]; try done.
+        case Hgt : vx => [gt|||||||||||||||||||||||||||||||||||||gt|gt|gt|gt|]; try done.
+        intros.
+        rewrite mem_seq1 in H0.
+        move /eqP : H0 => H0.
+        rewrite H0 in H1; clear H0.
+        case Hfill : (fillft_vm (tmap_type_size t_tgt) t_tgt v_tgt vmap) => [t_tgt'|]; rewrite Hfill in H; try done.
+        case Hfill2 : (fillft_vm (tmap_type_size t_src) t_src v_src vmap) => [t_src'|]; rewrite Hfill2 in H; try done.
+        apply ftype2fgtyp_non_passive_compatible with (n := (N.sub v.2 v_tgt.2)) in H; try done.
+        generalize Hsplit.
+        apply split_non_passive_flip_eq with (n := N.to_nat v.2 - N.to_nat v_tgt.2) (p := (refr, b)) in Hsplit; try done.
+        move => Hsplit'.
+        simpl in Hsplit.
+        rewrite <-Nnat.N2Nat.inj_sub in Hsplit; try done.
+        rewrite Nnat.N2Nat.id in Hsplit; try done.
+        assert (ftype_equiv t_tgt t_src).
+        admit.
+        apply ftype_eq_check_flip with (n := N.sub v.2 v_tgt.2) in H0.
+        rewrite -H0 in Hsplit; clear H0.
+        generalize Hfill.
+        apply fillft_vm_eq in Hfill.
+        apply ftype_eq_check_flip with (n := N.sub v.2 v_tgt.2) in Hfill.
+        rewrite Hfill in Hsplit; clear Hfill.
+        rewrite -Hsplit Hb in H.
+        case Htgtn : (ft_find_sub t_tgt' (v.2 - v_tgt.2)) => [gte|]; rewrite Htgtn in H.
+        apply component_vx_type_vm with (v := v) (vmap := vmap) (t_tgt' := t_tgt') (gte := gte) in Hbase; try done.
+        rewrite Hr in Hbase.
+        move => Hfill.
+        apply Hbase in Hfill; clear Hbase.
+        rewrite Hv Hgt in Hfill.
+        rewrite -Hfill in Htgtn H; clear Hfill.
+        apply fillft_vm_nth_eq with (r := r2) (rstl := rstl) (refr := refr) (b := b) (n := N.to_nat v.2 - N.to_nat v_tgt.2) (tmap := tmap) (gt := te) in Hfill2; try done.
+        rewrite <-Nnat.N2Nat.inj_sub in Hfill2; try done.
+        rewrite Nnat.N2Nat.id in Hfill2; try done.
+        rewrite Hfill2 in H; done.
+        done.
+        admit. (* None *)
+        (* 和上面一样的case *)
+        admit.
+        admit.
+        admit.
+        admit.
+      case Hr2 : (v.1 == v_src.1); try done.
+        (* rhs *)
+        case Hsplit : (split_expr_non_passive r t_tgt false) => [rstl|]; try done.
+        case Hnth : (nth_error rstl (N.to_nat v.2 - N.to_nat v_src.2)) => [[refr b]|]; try done.
+        case Hb : b; try done.
+        case Hv : (module_graph_vertex_set_p.find v vmap) => [vx|]; try done.
+        case Hgt : vx => [gt|||||||||||||||||||||||||||||||||||||gt|gt|gt|gt|]; try done.
+        intros.
+        rewrite mem_seq1 in H0.
+        move /eqP : H0 => H0.
+        rewrite H0 in H1; clear H0.
+        case Hfill : (fillft_vm (tmap_type_size t_tgt) t_tgt v_tgt vmap) => [t_tgt'|]; rewrite Hfill in H; try done.
+        case Hfill2 : (fillft_vm (tmap_type_size t_src) t_src v_src vmap) => [t_src'|]; rewrite Hfill2 in H; try done.
+        generalize Hfill.
+        apply ftype2fgtyp_non_passive_compatible with (n := (N.sub v.2 v_src.2)) in H; try done.
+        generalize Hsplit.
+        apply split_non_passive_flip_eq with (n := N.to_nat v.2 - N.to_nat v_src.2) (p := (refr, b)) in Hsplit; try done.
+        move => Hsplit'.
+        simpl in Hsplit.
+        rewrite <-Nnat.N2Nat.inj_sub in Hsplit; try done.
+        rewrite Nnat.N2Nat.id in Hsplit; try done.
+        apply fillft_vm_eq in Hfill.
+        apply ftype_eq_check_flip with (n := N.sub v.2 v_src.2) in Hfill.
+        rewrite Hfill in Hsplit; clear Hfill.
+        move => Hfill.
+        rewrite -Hsplit Hb in H.
+        case Hsrcn : (ft_find_sub t_src' (v.2 - v_src.2)) => [gte|]; rewrite Hsrcn in H.
+        apply component_vx_type_vm with (v := v) (vmap := vmap) (t_tgt' := t_src') (gte := gte) in Hbase2; try done.
+        rewrite Hr2 in Hbase2.
+        apply Hbase2 in Hfill2; clear Hbase2.
+        rewrite Hv Hgt in Hfill2.
+        rewrite -Hfill2 in Hsrcn H; clear Hfill2.
+        apply fillft_vm_nth_eq with (r := r) (rstl := rstl) (refr := refr) (b := b) (n := N.to_nat v.2 - N.to_nat v_src.2) (tmap := tmap) (gt := te) in Hfill; try done.
+        rewrite <-Nnat.N2Nat.inj_sub in Hfill; try done.
+        rewrite Nnat.N2Nat.id in Hfill; try done.
+        rewrite Hfill in H; done.
+        done.
+        admit. (* None *)
+        (* 和上面一样的case *)
+        admit.
+        admit.
+        admit.
+        admit.
+        case Hv : (module_graph_vertex_set_p.find v vmap) => [vx|]; try done.
+        case Hgt : vx => [gt|||||||||||||||||||||||||||||||||||||gt|gt|gt|gt|]; try done.
+        case Hv : (module_graph_vertex_set_p.find v vmap) => [vx|]; try done.
+        case Hgt : vx => [gt|||||||||||||||||||||||||||||||||||||gt|gt|gt|gt|]; try done.
+  - (* invalid *)
+    clear Sem_frag_stmts_correct4r.
+    case Hv : (module_graph_vertex_set_p.find v vmap) => [vx|]; try done.
+    case Hgt : vx => [gt|||||||||||||||||||||||||||||||||||||gt|gt|gt|gt|]; try done.
+  - (* when *)
+    move : H => [H0 H1].
+    apply Sem_frag_stmts_correct4r with (v := v) in H0.
+    case Hfind1 : (find_sub_exprs v s1 tmap) => [el1|]; rewrite Hfind1 in H0; try done.
+    apply Sem_frag_stmts_correct4r with (v := v) in H1.
+    case Hfind2 : (find_sub_exprs v s2 tmap) => [el2|]; rewrite Hfind2 in H1; try done.
+    case Hv : (module_graph_vertex_set_p.find v vmap) => [vx|]; rewrite Hv in H0 H1; try done.
+    case Hgt : vx => [gt|||||||||||||||||||||||||||||||||||||gt|gt|gt|gt|]; rewrite Hgt in H0 H1; try done.
+    intros.
+    rewrite mem_cat in H.
+    case Hin1 : (e \in el1); rewrite Hin1 in H.
+    apply H0 with (te := te) in Hin1; try done.
+    rewrite orb_false_l in H.
+    apply H1 with (te := te) in H; try done.
+    (* 一样的vx case *)
+    admit.
+    admit.
+    admit.
+    admit.
+
+  clear Sem_frag_stmts_correct4r.
+  elim.
+  admit.
+  intros hd tl IH vmap tmap Hsem v.
+  simpl.
+  simpl in Hsem.
+  move : Hsem => [Hsem0 Hsem].
+  apply Sem_frag_stmt_correct4r with (v := v) in Hsem0.
+  apply IH with (v := v) in Hsem.
+  case Hhd : (find_sub_expr v hd tmap) => [el1|]; rewrite Hhd in Hsem0; try done.
+  case Htl : (find_sub_exprs v tl tmap) => [el2|]; rewrite Htl in Hsem; try done.
+  case Hv : (module_graph_vertex_set_p.find v vmap) => [vx|]; rewrite Hv in Hsem0 Hsem; try done.
+  case Hgt : vx => [gt|||||||||||||||||||||||||||||||||||||gt|gt|gt|gt|]; rewrite Hgt in Hsem0 Hsem; try done.
+  intros.
+  rewrite mem_cat in H.
+  case Hin1 : (e \in el1); rewrite Hin1 in H.
+  apply Hsem0 with (te := te) in Hin1; try done.
+  rewrite orb_false_l in H.
+  apply Hsem with (te := te) in H; try done.
+  (* 一样的vx case *)
+  admit.
+  admit.
+  admit.
+  admit.
+Admitted.
+
+Lemma add_expr_connect_findn : forall (r v : ProdVarOrder.t) rstl (var2exprs0 : var2exprsmap), 
+  if (v.1 == r.1) then 
+    if (v.2 <= N.add r.2 (N.of_nat (List.length rstl))) 
+      then match module_graph_vertex_set_p.find v var2exprs0, List.nth_error rstl (N.to_nat (N.sub v.2 r.2)) with
+      | Some el0, Some e => module_graph_vertex_set_p.find v (add_expr_connect r rstl var2exprs0) = Some (e :: el0)
+      | None, Some e => module_graph_vertex_set_p.find v (add_expr_connect r rstl var2exprs0) = Some [::e]
+      | _,_ => module_graph_vertex_set_p.find v var2exprs0 = module_graph_vertex_set_p.find v (add_expr_connect r rstl var2exprs0)
+      end
+    else
+      module_graph_vertex_set_p.find v var2exprs0 = module_graph_vertex_set_p.find v (add_expr_connect r rstl var2exprs0)
+  else 
+    module_graph_vertex_set_p.find v var2exprs0 = module_graph_vertex_set_p.find v (add_expr_connect r rstl var2exprs0).
+Proof.
+Admitted.
+
+Lemma add_expr_non_passive_findn : forall (v v_tgt v_src : ProdVarOrder.t) lhsl rhsl (var2exprs0 var2exprs : var2exprsmap), 
+  add_expr_connect_non_passive v_tgt v_src lhsl rhsl var2exprs0 = Some var2exprs ->
+  if (v.1 == v_tgt.1) then 
+    if (v.2 <= N.add v_tgt.2 (N.of_nat (List.length rhsl))) 
+      then match module_graph_vertex_set_p.find v var2exprs0, List.nth_error rhsl (N.to_nat (N.sub v.2 v_tgt.2)) with
+      | Some el0, Some (e, false) => module_graph_vertex_set_p.find v var2exprs = Some ((Eref e) :: el0) 
+      | None, Some (e, false) => module_graph_vertex_set_p.find v var2exprs = Some [::(Eref e)] 
+      | _,_ => module_graph_vertex_set_p.find v var2exprs0 = module_graph_vertex_set_p.find v var2exprs
+      end
+    else
+    module_graph_vertex_set_p.find v var2exprs0 = module_graph_vertex_set_p.find v var2exprs
+  else if (v.1 == v_src.1) then
+    if (v.2 <= N.add v_src.2 (N.of_nat (List.length lhsl))) 
+      then match module_graph_vertex_set_p.find v var2exprs0, List.nth_error lhsl (N.to_nat (N.sub v.2 v_src.2)) with
+      | Some el0, Some (e, true) => module_graph_vertex_set_p.find v var2exprs = Some ((Eref e) :: el0) 
+      | None, Some (e, true) => module_graph_vertex_set_p.find v var2exprs = Some [::(Eref e)] 
+      | _,_ => module_graph_vertex_set_p.find v var2exprs0 = module_graph_vertex_set_p.find v var2exprs
+      end
+    else
+    module_graph_vertex_set_p.find v var2exprs0 = module_graph_vertex_set_p.find v var2exprs
+  else
+    module_graph_vertex_set_p.find v var2exprs0 = module_graph_vertex_set_p.find v var2exprs.
+Proof.
+Admitted.
+
+Lemma find_sub_expr_eq : forall s tmap0 tmap var2exprs0 var2exprs, stmt_tmap (tmap0, var2exprs0) s = Some (tmap, var2exprs) ->
+  forall (v : ProdVarOrder.t), match module_graph_vertex_set_p.find v var2exprs0, find_sub_expr v s tmap, module_graph_vertex_set_p.find v var2exprs with
+  | Some el0, Some el', Some el => TopoSort.subset el (el' ++ el0) /\ TopoSort.subset (el' ++ el0) el
+  | Some el0, None, Some el => TopoSort.subset el el0 /\ TopoSort.subset el0 el
+  | None, Some el', Some el => TopoSort.subset el el' /\ TopoSort.subset el' el
+  | None, Some nil, None => True
+  | None, None, None => True
+  | _,_, _ => False
+  end
+with find_sub_exprs_eq : forall ss tmap0 tmap var2exprs0 var2exprs, stmts_tmap (tmap0, var2exprs0) ss = Some (tmap, var2exprs) ->
+  forall (v : ProdVarOrder.t), match module_graph_vertex_set_p.find v var2exprs0, find_sub_exprs v ss tmap, module_graph_vertex_set_p.find v var2exprs with
+  | Some el0, Some el', Some el => TopoSort.subset el (el' ++ el0) /\ TopoSort.subset (el' ++ el0) el
+  | Some el0, None, Some el => TopoSort.subset el el0 /\ TopoSort.subset el0 el
+  | None, Some el', Some el => TopoSort.subset el el' /\ TopoSort.subset el' el
+  | None, Some nil, None => True
+  | None, None, None => True
+  | _,_, _ => False
+  end.
+Proof.
+  clear find_sub_expr_eq.
+  intros.
+  case Hs : s => [|r t|r reg|||r e|r e|r|c s1 s2]; rewrite Hs in H; simpl in H; simpl.
+  - (* skip *)
+    inversion H. 
+    case Hfind : (module_graph_vertex_set_p.find v var2exprs) => [el0|]; try done.
+    split; apply TopoSort.subset_refl.
+  - (* wire *)
+    case Hr : (CEP.find r tmap0); rewrite Hr in H; try discriminate.
+    inversion H.
+    case Hfind : (module_graph_vertex_set_p.find v var2exprs) => [el0|]; try done.
+    split; apply TopoSort.subset_refl.
+  - (* reg *)
+    clear find_sub_exprs_eq.
+    case Hr : (CEP.find r tmap0); rewrite Hr in H; try discriminate.
+    case Hrst : (reset reg) => [|rst_sig rst_val]; rewrite Hrst in H.
+    inversion H.
+    case Hfind : (module_graph_vertex_set_p.find v var2exprs) => [el0|]; try done.
+    case : (v.1 == r.1); simpl; split; apply TopoSort.subset_refl.
+    case : (v.1 == r.1); simpl; done.
+    case Hsplit : (split_expr_connect rst_val (type reg)) => [rstl|]; rewrite Hsplit in H; try discriminate.
+    inversion H; clear H.
+    specialize add_expr_connect_findn with (r := r) (v := v) (rstl := rstl) (var2exprs0 := var2exprs0); intro.
+    case Hv : (v.1 == r.1); rewrite Hv in H.
+    assert (Hv2 : v.2 <= (N.of_nat (length rstl))).
+    admit.
+    assert (r.2 = N0).
+    admit.
+    rewrite H0 in H; clear H0.
+    rewrite Hv2 in H.
+    case Hfind0 : (module_graph_vertex_set_p.find v var2exprs0) => [el0|]; rewrite Hfind0 in H.
+    assert ((N.to_nat (v.2 - 0)) = (N.to_nat v.2)).
+    admit.
+    rewrite H0 in H; clear H0.
+    case Hnth : (nth_error rstl (N.to_nat v.2)) => [e|]; rewrite Hnth in H.
+    rewrite H.
+    assert ((e :: el0) = ([:: e] ++ el0)).
+    simpl; done.
+    rewrite H0.
+    split; rewrite TopoSort.subset_refl; done.
+    rewrite -H.
+    split; rewrite TopoSort.subset_refl; done.
+    assert ((N.to_nat (v.2 - 0)) = (N.to_nat v.2)).
+    admit.
+    rewrite H0 in H; clear H0.
+    case Hnth : (nth_error rstl (N.to_nat v.2)) => [e|]; rewrite Hnth in H.
+    rewrite H.
+    simpl.
+    rewrite mem_seq1.
+    rewrite eq_refl; done.
+    rewrite -H; done.
+    case Hfind0 : (module_graph_vertex_set_p.find v var2exprs0) => [el0|]; rewrite Hfind0 in H.
+    rewrite -H.
+    simpl.
+    split; rewrite TopoSort.subset_refl; done.
+    rewrite -H; done.
+  discriminate.
+  discriminate.
+  - (* node *)
+    clear find_sub_exprs_eq.
+    case Hr : (CEP.find r tmap0); rewrite Hr in H; try discriminate.
+    case Hte : (type_of_hfexpr e tmap0) => [te|]; rewrite Hte in H; try discriminate.
+    case Hsplit : (split_expr_connect e te) => [rstl|]; rewrite Hsplit in H; try discriminate.
+    inversion H.
+    case Hfind : (module_graph_vertex_set_p.find v var2exprs0) => [el0|]; try done.
+    specialize add_expr_connect_findn with (r := r) (v := v) (rstl := rstl) (var2exprs0 := var2exprs0); intro.
+    case Hv : (v.1 == r.1); rewrite Hv in H0.
+    assert (Hv2 : v.2 <= (N.of_nat (length rstl))).
+    admit.
+    assert (r.2 = N0).
+    admit.
+    rewrite H3 in H0.
+    rewrite Hv2 in H0.
+    rewrite Hfind in H0.
+    assert (r = (r.1, N0)).
+    rewrite -H3.
+    apply surjective_pairing.
+    rewrite {1}H4; clear H4 H3.
+    rewrite type_of_hfexpr_eq Hte Hsplit.
+    assert ((N.to_nat (v.2 - 0)) = (N.to_nat v.2)).
+    admit.
+    rewrite H3 in H0; clear H3.
+    case Hnth : (nth_error rstl (N.to_nat v.2)) => [e0|]; rewrite Hnth in H0.
+    rewrite H0.
+    assert ((e0 :: el0) = ([:: e0] ++ el0)).
+    simpl; done.
+    rewrite H3.
+    split; rewrite TopoSort.subset_refl; done.
+    rewrite -H0.
+    split; rewrite TopoSort.subset_refl; done.
+    rewrite -H0 Hfind.
+    simpl; rewrite TopoSort.subset_refl; done.
+    specialize add_expr_connect_findn with (r := r) (v := v) (rstl := rstl) (var2exprs0 := var2exprs0); intro.
+    case Hv : (v.1 == r.1); rewrite Hv in H0.
+    assert (Hv2 : v.2 <= (N.of_nat (length rstl))).
+    admit.
+    assert (r.2 = N0).
+    admit.
+    rewrite H3 in H0.
+    rewrite Hv2 in H0.
+    rewrite Hfind in H0.
+    assert (r = (r.1, N0)).
+    rewrite -H3.
+    apply surjective_pairing.
+    rewrite {1}H4; clear H4 H3.
+    rewrite type_of_hfexpr_eq Hte Hsplit.
+    assert ((N.to_nat (v.2 - 0)) = (N.to_nat v.2)).
+    admit.
+    rewrite H3 in H0; clear H3.
+    case Hnth : (nth_error rstl (N.to_nat v.2)) => [e0|]; rewrite Hnth in H0.
+    rewrite H0.
+    rewrite TopoSort.subset_refl; done.
+    rewrite -H0; done.
+    rewrite -H0 Hfind; done.
+  - (* fcnct *)
+    clear find_sub_exprs_eq.
+    case He : e =>[t c| c e1 | u e1 | op e1 e2 | c e1 e2 | c e1 | r2 ]; rewrite He in H; try done.
+    (* 一般connection *)
+    rewrite -He; rewrite -He in H.
+    case Hbase : (base_ref r tmap0) => [[v_tgt t_tgt]|]; rewrite Hbase in H; try discriminate.
+    case Hte : (type_of_hfexpr e tmap0) => [t_src|]; rewrite Hte in H; try discriminate.
+    case Hconnect : (connect_type_compatible t_tgt t_src); rewrite Hconnect in H; try discriminate.
+    case Hsplit : (split_expr_connect e t_src) => [rstl|]; rewrite Hsplit in H; try discriminate.
+    inversion H; clear H.
+    specialize add_expr_connect_findn with (r := v_tgt) (v := v) (rstl := rstl) (var2exprs0 := var2exprs0); intro.
+    case Hv : (v.1 == v_tgt.1); rewrite Hv in H.
+    case Hv2 : (v.2 <= N.add v_tgt.2 (N.of_nat (length rstl))); rewrite Hv2 in H.
+    case Hfind0 : (module_graph_vertex_set_p.find v var2exprs0) => [el0|]; rewrite Hfind0 in H.
+    rewrite -H1 Hbase Hte Hv Hsplit.
+    rewrite <-Nnat.N2Nat.inj_sub.
+    case Hnth : (nth_error rstl (N.to_nat (v.2 - v_tgt.2))) => [e0|]; rewrite Hnth in H.
+    rewrite H.
+    assert ((e0 :: el0) = ([:: e0] ++ el0)).
+    simpl; done.
+    rewrite H0.
+    split; rewrite TopoSort.subset_refl; done.
+    rewrite -H.
+    split; rewrite TopoSort.subset_refl; done.
+      (* the same *)
+      rewrite -H1 Hbase Hte Hv Hsplit.
+      rewrite <-Nnat.N2Nat.inj_sub.
+      case Hnth : (nth_error rstl (N.to_nat (v.2 - v_tgt.2))) => [e0|]; rewrite Hnth in H.
+      rewrite H.
+      split; rewrite TopoSort.subset_refl; done.
+      rewrite -H.
+      split; rewrite TopoSort.subset_refl; done.
+    case Hfind0 : (module_graph_vertex_set_p.find v var2exprs0) => [el0|]; rewrite Hfind0 in H.
+    rewrite -H1 Hbase Hte Hv Hsplit.
+    rewrite <-Nnat.N2Nat.inj_sub.
+    assert (nth_error rstl (N.to_nat (v.2 - v_tgt.2)) = None).
+    admit. (* v.2超出range *)
+    rewrite H0 -H.
+    split; rewrite TopoSort.subset_refl; done.
+    rewrite -H1 Hbase Hte Hv Hsplit.
+    rewrite <-Nnat.N2Nat.inj_sub.
+    assert (nth_error rstl (N.to_nat (v.2 - v_tgt.2)) = None).
+    admit. (* v.2超出range *)
+    rewrite H0 - H; done.
+    case Hfind0 : (module_graph_vertex_set_p.find v var2exprs0) => [el0|]; rewrite Hfind0 in H.
+    rewrite -H1 Hbase Hte Hv.
+    rewrite -H.
+    simpl.
+    split; rewrite TopoSort.subset_refl; done.
+    rewrite -H1 Hbase Hte Hv.
+    rewrite -H.
+    simpl.
+    split; rewrite TopoSort.subset_refl; done.
+    (* 同上的connection case *)
+    admit.
+    admit.
+    admit.
+    admit.
+    admit.
+    (* Eref connection *)
+    case Hbase : (base_ref r tmap0) => [[v_tgt t_tgt]|]; rewrite Hbase in H; try discriminate.
+    case Hbase2 : (base_ref r2 tmap0) => [[v_src t_src]|]; rewrite Hbase2 in H; try discriminate.
+    case Hsplit : (split_expr_non_passive r t_tgt false) => [lhsl|]; rewrite Hsplit in H; try discriminate.
+    case Hsplit2 : (split_expr_non_passive r2 t_src false) => [rhsl|]; rewrite Hsplit2 in H; try discriminate.
+    case Hadd : (add_expr_connect_non_passive v_tgt v_src lhsl rhsl var2exprs0) => [newv2e|]; rewrite Hadd in H; try discriminate.
+    inversion H; clear H.
+    rewrite H2 in Hadd; clear H2 newv2e.
+    rewrite -H1 Hbase Hbase2 Hsplit2 Hsplit.
+    apply add_expr_non_passive_findn with (v := v) (v_tgt := v_tgt) (v_src := v_src) (lhsl := lhsl) (rhsl := rhsl) (var2exprs0 := var2exprs0) (var2exprs := var2exprs) in Hadd.
+    (* Nflip *)
+    case Hv : (v.1 == v_tgt.1); rewrite Hv in Hadd.
+    case Hv2 : (v.2 <= N.add v_tgt.2 (N.of_nat (length rhsl))); rewrite Hv2 in Hadd.
+    case Hfind0 : (module_graph_vertex_set_p.find v var2exprs0) => [el0|]; rewrite Hfind0 in Hadd.
+    rewrite <-Nnat.N2Nat.inj_sub.
+    case Hnth : (nth_error rhsl (N.to_nat (v.2 - v_tgt.2))) => [[refr b]|]; rewrite Hnth in Hadd.
+    case Hb : b; rewrite Hb in Hadd; try done.
+    rewrite -Hadd.
+    split; rewrite TopoSort.subset_refl; done.
+    rewrite Hadd.
+    assert ((Eref refr :: el0) = ([:: Eref refr] ++ el0)).
+    simpl; done.
+    rewrite H.
+    split; rewrite TopoSort.subset_refl; done.
+    rewrite -Hadd.
+    split; rewrite TopoSort.subset_refl; done.
+      (* the same case *)
+      rewrite <-Nnat.N2Nat.inj_sub.
+      case Hnth : (nth_error rhsl (N.to_nat (v.2 - v_tgt.2))) => [[refr b]|]; rewrite Hnth in Hadd.
+      case Hb : b; rewrite Hb in Hadd; try done.
+      rewrite -Hadd; done.
+      rewrite Hadd.
+      split; rewrite TopoSort.subset_refl; done.
+      rewrite -Hadd; done.
+    case Hfind0 : (module_graph_vertex_set_p.find v var2exprs0) => [el0|].
+    assert (nth_error rhsl (N.to_nat v.2 - N.to_nat v_tgt.2) = None).
+    admit.
+    rewrite H; clear H.
+    rewrite -Hadd Hfind0.
+    split; rewrite TopoSort.subset_refl; done.
+    assert (nth_error rhsl (N.to_nat v.2 - N.to_nat v_tgt.2) = None).
+    admit.
+    rewrite H; clear H.
+    rewrite -Hadd Hfind0; done.
+    (* flipped *)
+    clear Hv.
+    case Hv : (v.1 == v_src.1); rewrite Hv in Hadd.
+    case Hv2 : (v.2 <= N.add v_src.2 (N.of_nat (length lhsl))); rewrite Hv2 in Hadd.
+    case Hfind0 : (module_graph_vertex_set_p.find v var2exprs0) => [el0|]; rewrite Hfind0 in Hadd.
+    rewrite <-Nnat.N2Nat.inj_sub.
+    case Hnth : (nth_error lhsl (N.to_nat (v.2 - v_src.2))) => [[refl b]|]; rewrite Hnth in Hadd.
+    case Hb : b; rewrite Hb in Hadd; try done.
+    rewrite Hadd.
+    assert ((Eref refl :: el0) = ([:: Eref refl] ++ el0)).
+    simpl; done.
+    rewrite H.
+    split; rewrite TopoSort.subset_refl; done.
+    rewrite -Hadd.
+    split; rewrite TopoSort.subset_refl; done.
+    rewrite -Hadd.
+    split; rewrite TopoSort.subset_refl; done.
+      (* the same case *)
+      rewrite <-Nnat.N2Nat.inj_sub.
+      case Hnth : (nth_error lhsl (N.to_nat (v.2 - v_src.2))) => [[refl b]|]; rewrite Hnth in Hadd.
+      case Hb : b; rewrite Hb in Hadd; try done.
+      rewrite Hadd.
+      split; rewrite TopoSort.subset_refl; done.
+      rewrite -Hadd; done.
+      rewrite -Hadd; done.
+    case Hfind0 : (module_graph_vertex_set_p.find v var2exprs0) => [el0|].
+    assert (nth_error lhsl (N.to_nat v.2 - N.to_nat v_src.2) = None).
+    admit.
+    rewrite H; clear H.
+    rewrite -Hadd Hfind0.
+    split; rewrite TopoSort.subset_refl; done.
+    assert (nth_error lhsl (N.to_nat v.2 - N.to_nat v_src.2) = None).
+    admit.
+    rewrite H; clear H.
+    rewrite -Hadd Hfind0; done.
+    case Hfind0 : (module_graph_vertex_set_p.find v var2exprs0) => [el0|].
+    rewrite -Hadd Hfind0; simpl.
+    split; rewrite TopoSort.subset_refl; done.
+    rewrite -Hadd Hfind0; done.
+  - (* invalid *)
+    inversion H. 
+    case Hfind : (module_graph_vertex_set_p.find v var2exprs) => [el0|]; try done.
+    split; apply TopoSort.subset_refl.
+  - (* when *)
+    case Hstmts : (stmts_tmap (tmap0, var2exprs0) s1) => [[tmap' var2exprs']|]; rewrite Hstmts in H. 
+    apply find_sub_exprs_eq with (v := v) in Hstmts.
+    apply find_sub_exprs_eq with (v := v) in H; clear find_sub_exprs_eq.
+    case Hfind0 : (module_graph_vertex_set_p.find v var2exprs0) => [el0|]; rewrite Hfind0 in Hstmts; try done.
+    case Hfind' : (module_graph_vertex_set_p.find v var2exprs') => [el'|]; rewrite Hfind' in H; try done.
+    assert (find_sub_exprs v s1 tmap = find_sub_exprs v s1 tmap').
+    admit.
+    case Hexpr1 : (find_sub_exprs v s1 tmap) => [e1|]; rewrite -H0 Hexpr1 Hfind' in Hstmts.
+    case Hexpr2 : (find_sub_exprs v s2 tmap) => [e2|]; rewrite Hexpr2 in H.
+    case Hfind : (module_graph_vertex_set_p.find v var2exprs) => [el|]; rewrite Hfind in H; try done.
+    admit.
+    admit. (* 不是None *)
+    admit. (* 不是None *)
+    assert (find_sub_exprs v s1 tmap = find_sub_exprs v s1 tmap').
+    admit.
+    case Hexpr1 : (find_sub_exprs v s1 tmap) => [e1|]; rewrite -H0 Hexpr1 Hfind' in Hstmts.
+    case Hexpr2 : (find_sub_exprs v s2 tmap) => [e2|]; rewrite Hexpr2 in H.
+    case Hfind : (module_graph_vertex_set_p.find v var2exprs) => [el|]; rewrite Hfind in H; try done.
+    done.
+    done.
+    (* same case *)
+      case Hfind' : (module_graph_vertex_set_p.find v var2exprs') => [el'|]; rewrite Hfind' in H; try done.
+      assert (find_sub_exprs v s1 tmap = find_sub_exprs v s1 tmap').
+      admit.
+      case Hexpr1 : (find_sub_exprs v s1 tmap) => [e1|]; rewrite -H0 Hexpr1 Hfind' in Hstmts.
+      case Hexpr2 : (find_sub_exprs v s2 tmap) => [e2|]; rewrite Hexpr2 in H.
+      case Hfind : (module_graph_vertex_set_p.find v var2exprs) => [el|]; rewrite Hfind in H; try done.
+      admit.
+      admit. (* 不是None *)
+      done.
+      assert (find_sub_exprs v s1 tmap = find_sub_exprs v s1 tmap').
+      admit.
+      case Hexpr1 : (find_sub_exprs v s1 tmap) => [e1|]; rewrite -H0 Hexpr1 Hfind' in Hstmts.
+      case Hexpr2 : (find_sub_exprs v s2 tmap) => [e2|]; rewrite Hexpr2 in H.
+      case Hfind : (module_graph_vertex_set_p.find v var2exprs) => [el|]; rewrite Hfind in H; try done.
+      case He1 : e1; rewrite He1 in Hstmts; try done.
+      case He1 : e1; rewrite He1 in Hstmts; try done.
+      case He1 : e1; rewrite He1 in Hstmts; try done.
+      admit. (* 不是None *)
+      discriminate.
+
+  clear find_sub_exprs_eq.
+  elim.
+  admit.
+  intros hd tl IH tmap0 tmap var2exprs0 var2exprs H v.
+  simpl in H.
+  case Hstmts : (stmt_tmap (tmap0, var2exprs0) hd) => [[tmap' var2exprs']|]; rewrite Hstmts in H. 
+  apply find_sub_expr_eq with (v := v) in Hstmts.
+  apply IH with (v := v) in H; clear find_sub_expr_eq.
+  case Hfind0 : (module_graph_vertex_set_p.find v var2exprs0) => [el0|]; rewrite Hfind0 in Hstmts; try done; simpl.
+  case Hfind' : (module_graph_vertex_set_p.find v var2exprs') => [el'|]; rewrite Hfind' in H; try done; simpl.
+  assert (find_sub_expr v hd tmap = find_sub_expr v hd tmap').
+  admit.
+  case Hexpr1 : (find_sub_expr v hd tmap) => [e1|]; rewrite -H0 Hexpr1 Hfind' in Hstmts.
+  case Hexpr2 : (find_sub_exprs v tl tmap) => [e2|]; rewrite Hexpr2 in H.
+  case Hfind : (module_graph_vertex_set_p.find v var2exprs) => [el|]; rewrite Hfind in H; try done.
+  admit.
+  admit. (* 不是None *)
+  admit. (* 不是None *)
+  case Hexpr1 : (find_sub_expr v hd tmap') => [e1|]; rewrite Hexpr1 Hfind' in Hstmts; try done.
+  assert (find_sub_expr v hd tmap = find_sub_expr v hd tmap').
+  admit.
+    (* same case *)
+    case Hfind' : (module_graph_vertex_set_p.find v var2exprs') => [el'|]; rewrite Hfind' in H; try done.
+    assert (find_sub_expr v hd tmap = find_sub_expr v hd tmap').
+    admit.
+    case Hexpr1 : (find_sub_expr v hd tmap) => [e1|]; rewrite -H0 Hexpr1 Hfind' in Hstmts; try done.
+    case Hexpr2 : (find_sub_exprs v tl tmap) => [e2|]; rewrite Hexpr2 in H; try done.
+    case Hfind : (module_graph_vertex_set_p.find v var2exprs) => [el|]; rewrite Hfind in H; try done.
+    admit.
+    admit. (* 不是None *)
+      assert (find_sub_exprs v s1 tmap = find_sub_exprs v s1 tmap').
+      admit.
+      case Hexpr1 : (find_sub_exprs v s1 tmap) => [e1|]; rewrite -H0 Hexpr1 Hfind' in Hstmts.
+      case Hexpr2 : (find_sub_exprs v s2 tmap) => [e2|]; rewrite Hexpr2 in H.
+      case Hfind : (module_graph_vertex_set_p.find v var2exprs) => [el|]; rewrite Hfind in H; try done.
+      case He1 : e1; rewrite He1 in Hstmts; try done.
+      case He1 : e1; rewrite He1 in Hstmts; try done.
+      case He1 : e1; rewrite He1 in Hstmts; try done.
+      admit. (* 不是None *)
+      discriminate.
+Admitted.
+
+Lemma InferWidths_fun_correct' : forall (vmap : module_graph_vertex_set_p.env) (var2exprs : var2exprsmap) (tmap : CEP.t ftype) (pp : seq HiFP.hfport) (ss : HiFP.hfstmt_seq), 
+  stmts_tmap (ports_tmap pp, module_graph_vertex_set_p.empty (seq HiFP.hfexpr)) ss = Some (tmap, var2exprs) ->
+  Sem_frag_stmts' vmap ss tmap -> 
+  forall (v : ProdVarOrder.t), match module_graph_vertex_set_p.find v vmap with
+  | Some (OutPort gt) 
+  | Some (Register gt) 
+  | Some (RegisterReset gt _) 
+  | Some (Wire gt) 
+  | Some (Node gt) => match module_graph_vertex_set_p.find v var2exprs, CEP.find (fst v, N0) tmap with
+                    | Some el, Some init => match fil_ftlist (map (fun e => type_of_hfexpr_vm vmap e tmap) el), ft_find_sub init v.2 with
+                                | Some eftl, Some initt => if (not_implicit gt) then true else
+                                                          match max_ftlist eftl initt with
+                                                          | Some nt => sizeof_fgtyp gt >= sizeof_fgtyp nt
+                                                          | _ => true
+                                                          end
+                                | _,_ => true
+                                end
+                    | _,_ => true
+                    end
+  | _ => true
+  end.
+Proof.
+  intros vmap var2exprs tmap pp ss Hprepro Hsem v.
+  apply Sem_frag_stmts_correct4r with (v := v) in Hsem.
+  case Hvx : (module_graph_vertex_set_p.find v vmap) => [vx|]; rewrite Hvx in Hsem; try done.
+  case Hgt : vx => [gt|||||||||||||||||||||||||||||||||||||gt|gt|gt|gt|]; rewrite Hgt in Hsem; try done.
+  apply find_sub_exprs_eq with (v := v) in Hprepro.
+  case Hel : (module_graph_vertex_set_p.find v var2exprs) => [el|]; rewrite Hel in Hprepro; try done.
+
+  case Hinit : (CEP.find (v.1, 0%num) tmap) => [init|]; try done.
+  case Hfil : (fil_ftlist [seq type_of_hfexpr_vm vmap e tmap | e <- el]) => [eftl|]; try done.
+  case Hinitt : (ft_find_sub init v.2) => [initt|]; try done.
+  case Himpli : (not_implicit gt); try done.
+  case Hmax : (max_ftlist eftl initt) => [nt|]; try done.
+  apply geq_conj2mux with (vmap := vmap) (tmap := tmap) (initt := initt) (el := el) (eftl := eftl); try done.
+
+  case Hel' : (find_sub_exprs v ss tmap) => [el'|]; rewrite Hel' in Hsem Hprepro; try done.
+  intros texpr tge Hin Htge.
+  apply Hsem in Htge.
+  rewrite /connect_fgtyp_compatible Himpli in Htge.
+  move /andP : Htge => [Htge _]; done.
+  move : Hprepro => [Hprepro _]. 
+  apply TopoSort.in_subset_trans with (x := texpr) in Hprepro; try done.
+
+  admit. (* 最初tmap中应该所有implicit为0 *)
+
+  (*assert (exists t0, Qin (@Swire ProdVarOrder.T (v.1, N0) t0) ss).
+
+   assert (((Finput (v.1, N0) init) \in pp) \/ 
+          (Qin (Swire (v.1, N0) init) ss \/
+          (exists reg0, Qin (Sreg (v.1, N0) reg0) ss /\ (type reg0 = init)) \/
+          (exists e0, Qin (Snode (v.1, N0) e0) ss /\ (type_of_hfexpr_vm vmap e0 tmap = init))).
+  *) (* 但也可能存在在when？ *)
+
+  
+
+  (* case1 : 是flip的v *)
+  (*assert (forall texpr, texpr \in el -> 
+  (exists r0 r1 v_ref rhsl, base_ref r1 tmap = Some v_ref -> split_expr_non_passive r0 v_ref.2 = Some lhsl -> 
+                 (v_ref.1.1 = v.1) /\ (List.nth_error lhsl (N.to_nat (N.sub v.2 v_ref.1.2)) = Some (texpr, true)) /\ (Qin (Sfcnct r0 (Eref r1)) ss))).
+  *)
+  admit.
+
+  (* case2 : 不是flip的v *)
+  (*assert (forall texpr, texpr \in el -> 
+  (exists r0 e0 v_ref el, base_ref r0 tmap = Some v_ref -> split_expr_connect e0 v_ref.2 = Some el -> 
+                 (v_ref.1.1 = v.1) /\ (List.nth_error el (N.to_nat (N.sub v.2 v_ref.1.2)) = Some texpr) /\ (Qin (Snode r0 e0) ss)) \/
+  (exists r0 r1 v_ref rhsl, base_ref r0 tmap = Some v_ref -> split_expr_non_passive r1 v_ref.2 = Some rhsl -> 
+                 (v_ref.1.1 = v.1) /\ (List.nth_error rhsl (N.to_nat (N.sub v.2 v_ref.1.2)) = Some (texpr, false)) /\ (Qin (Sfcnct r0 (Eref r1)) ss)) \/
+  (exists r0 e0 v_ref el, base_ref r0 tmap = Some v_ref -> split_expr_connect e0 v_ref.2 = Some el -> 
+                 (v_ref.1.1 = v.1) /\ (List.nth_error el (N.to_nat (N.sub v.2 v_ref.1.2)) = Some texpr) /\ (Qin (Sfcnct r0 e0) ss))).
+  *) (* ??报错 *)
+
+Admitted.
+
+Theorem InferWidths_correct' :
+  forall (F : HiFP.hfmodule) (vm' : module_graph_vertex_set_p.env) (ct : module_graph_connection_trees_p.env),
+    match InferWidths_m F with
+    | Some F' => Sem F' vm' ct -> Sem F (make_vm_implicit F vm') ct
+    | _ => True
+    end.
+Proof.
+  assert (Sem F' vm' ct -> Sem_frag_stmts' vm' ss tmap).
+  assert (Sem_frag_stmts' vm' ss tmap -> InferWidths_fun inferorder var2exprs tmap = Some newtm -> Sem_frag_stmts' vm' ss' tmap).
+  assert (Sem F' vm' ct -> Sem_frag_stmts' vm' ss' tmap -> Sem F (make_vm_implicit F vm') ct).
